WIP: Improved API for easier modification
This is a big patch but the main changes are:
- Replaced Std.Sat.Aig as the backing store - this means we can now
  modify nodes/no longer have to have dependently typed constraints on
  the and gate inputs
- added `Aig.inputs`/`Aig.latches`/`Aig.nodes` as abstracted
  representations of the respective aspects of the aig. This makes it
  easier to write theorems for them without having to repeatedly write
  out the effect on every getter. These are backed by a new `Utils.Map`
  type which represents an abstract hashmap type collection with a
  validity predicate, map from keys to values and size.
- Added new accessors/modifiers for updating the aig to allow things
  like converting between different nodes types

- Things broken by this that still need repairing in particular:
  - The iterators
  - The semantics definitions
  - Getting to/from Std.Sat.Aig

Valaig/Aig/Basic.lean
@@ -1,17 +1,16 @@
 module
 
-public import Std.Sat.AIG.Basic
-public import Std.Sat.AIG.CachedGates
 public meta import Valaig.Prelude
 public import Valaig.Utils.Pool
-public import Valaig.Aig.StdSatLemmas
+public import Valaig.Utils.Map
 public import Valaig.Aig.Refs
 public import Valaig.ForStd
 
+public section
 namespace Valaig.Aig
 
 /--
-The metadata of an input in the Aig.
+  The metadata of an input in the Aig.
 -/
 structure Input where
   var : Var
@@ -21,7 +20,12 @@ deriving instance Hashable, DecidableEq, Repr, Inhabited for Input
 end Input
 
 /--
-The metadata of a latch in the Aig.
+  We require the inputs we store in the array to only track non-constant indices.
+-/
+private abbrev InputData := { input : Input // input.var ≠ .constant }
+
+/--
+  The metadata of a latch in the Aig.
 -/
 structure Latch where
   var : Var
@@ -32,14 +36,17 @@ namespace Latch
 deriving instance Hashable, DecidableEq, Repr, Inhabited for Latch
 end Latch
 
+/--
+  We require the inputs we store in the array to only track non-constant indices.
+-/
+private abbrev LatchData := { latch : Latch // latch.var ≠ .constant }
+
 end Valaig.Aig
 
--- Switch to public
-public section
 namespace Valaig.Aig
 
 /--
-An index to an input definition in the Aig input pool. These inputs are primary inputs (PIs).
+  An index to an input definition in the Aig. These inputs are primary inputs (PIs).
 -/
 @[ext, grind ext]
 structure InputIdx where
@@ -53,7 +60,7 @@ instance : LawfulHashable InputIdx where hash_eq := by simp
 end InputIdx
 
 /--
-An index to a latch definition in the Aig latch pool.
+  An index to a latch definition in the Aig.
 -/
 @[ext, grind ext]
 structure LatchIdx where
@@ -67,9 +74,9 @@ instance : LawfulHashable LatchIdx where hash_eq := by simp
 end LatchIdx
 
 /--
-A leaf in the combinational aig is either an input or a latch, which is just a reference back to
-the index in the inputs or latches pools.
-These are what abc calls Combinational Inputs (CIs).
+  A leaf in the Aig is either an input or a latch, which is a reference back to the index
+  in the inputs or latches.
+  These are what abc calls Combinational Inputs (CIs).
 -/
 inductive LeafIdx where
 | input (idx : InputIdx)
@@ -90,8 +97,96 @@ instance : Coe LatchIdx LeafIdx where
 end LeafIdx
 
 /--
-An output of interest in the circuit - this is also used to represent other
-nameable nodes in the Aiger format like bad and constraint nodes.
+  A representation of the node data stored for a particular variable in an `Aig`. For inputs and
+  latches this requires a further lookup with `InputIdx.get` or `LatchIdx.get`.
+-/
+inductive Node where
+  | false
+  | input (idx : InputIdx)
+  | latch (idx : LatchIdx)
+  | and (lhs rhs : Lit)
+
+@[always_inline]
+instance : Coe InputIdx Node where
+  coe := (.input ·)
+
+@[always_inline]
+instance : Coe LatchIdx Node where
+  coe := (.latch ·)
+
+@[always_inline]
+instance : Coe LeafIdx Node where
+  coe
+  | .input idx
+  | .latch idx => idx
+
+namespace Node
+deriving instance Hashable, DecidableEq, Repr, Inhabited for Node
+end Node
+
+/--
+  The generic representation of nodes in the Aig, including inputs, latches and
+  gates. These are interpreted relative to their position in the Aig to give
+  semantics, see `NodeData.toNode`.
+-/
+private abbrev NodeData := Lit × Lit
+
+namespace NodeData
+
+private def false : NodeData :=
+  (.false, .false)
+
+@[always_inline, local simp, local grind]
+private def input (idx : InputIdx) (var : Var) : NodeData :=
+  (var.toLit .false, .ofIdx idx.idx)
+
+@[always_inline, local simp, local grind]
+private def latch (idx : LatchIdx) (var : Var) : NodeData :=
+  (var.toLit .true, .ofIdx idx.idx)
+
+@[always_inline, local simp, local grind]
+private def and (rhs0 rhs1 : Lit) : NodeData :=
+  (rhs0, rhs1)
+
+@[always_inline, local simp, local grind]
+private def toNode (data : NodeData) (var : Var) : Node :=
+  if var = .constant then
+    .false
+  else if data.fst.var = var then
+    if !data.fst.inverted then
+      .input <| .ofIdx data.snd.idx
+    else
+      .latch <| .ofIdx data.snd.idx
+  else
+    .and data.fst data.snd
+
+@[simp, grind =]
+private theorem toNode_constant {data : NodeData} :
+    data.toNode .constant = .false := by
+  simp
+
+@[simp, grind =]
+private theorem toNode_input {idx : InputIdx} {var : Var} (notConst : var ≠ .constant) :
+    (input idx var).toNode var = idx := by
+  grind
+
+@[simp, grind =]
+private theorem toNode_latch {idx : LatchIdx} {var : Var} (notConst : var ≠ .constant) :
+    (latch idx var).toNode var = idx := by
+  grind
+
+set_option linter.unusedVariables false in
+@[simp, grind =]
+private theorem toNode_and {rhs0 rhs1 : Lit} {var : Var} (notConst : var ≠ .constant)
+    (h0 : rhs0.var ≠ var) (h1 : rhs1.var ≠ var) :
+    (and rhs0 rhs1).toNode var = .and rhs0 rhs1 := by
+  grind
+
+end NodeData
+
+/--
+  An output of interest in the circuit - this is also used to represent other
+  referenced nodes in the Aiger format like bad and constraint nodes.
 -/
 structure Output where
   lit : Lit
@@ -105,97 +200,188 @@ abbrev Outputs := Array Output
 end Aig
 
 /--
-A sequential And-Inverter Graph consisting of inputs, latches and And gates. Outputs should be
-stored separately as `Lit`s in the `Aig`.
+  A sequential And-Inverter Graph consisting of inputs, latches and And gates.
 -/
 structure Aig where
-  -- The underlying AIG
-  private aig : Std.Sat.AIG Aig.LeafIdx
+  /-- The core array of nodes making up the Aig. -/
+  private _nodes : Array Aig.NodeData
 
-  -- This is a temporary constraint, later we will enforce this by simply not storing a false node
-  -- in the aig and always treating the constant variable as referring to false
-  private hconst :
-    ∀ (idx : Nat) (valid : idx < aig.decls.size),
-      aig.decls[idx] = .false ↔ idx = 0
+  /-- A mapping from input indices (`InputIdx`) to their definition. -/
+  private _inputs : Utils.Pool Aig.InputData
 
-  -- A mapping from input indices (LeafIdx.input idx) to their definition
-  private _inputs : Utils.Pool Aig.Input
+  /-- A mapping from latch indices (`LatchIdx`) to their definition. -/
+  private _latches : Utils.Pool Aig.LatchData
 
-  -- A mapping from latch indices (LeafIdx.latch idx) to their definition
-  private _latches : Utils.Pool Aig.Latch
+  /--
+    We always store at least one element, which regardless of value represents the constant false.
+  -/
+  private sized : _nodes.size > 0
 
 variable {aig : Aig}
 
 namespace Aig
 
 /--
-A representation of the node data stored for a particular variable in an `Aig`. For inputs and
-latches this requires a further lookup with `InputIdx.get` or `LatchIdx.get`.
+  A general error type for fallible Aig functions.
 -/
-inductive Node where
-  | false
-  | input (idx : InputIdx)
-  | latch (idx : LatchIdx)
-  | and (lhs rhs : Lit)
+inductive Err
+/-- Returned by `function!` functions if argument `arg` is invalid in the Aig when it is expected to be valid. -/
+| invalidIdx (function : String) (arg : String)
+/-- Generic error messages with an associated function. `Err.str` can be used to avoid defining a function location. -/
+| other (function : String) (msg : String)
 
-namespace Node
-deriving instance Hashable, DecidableEq, Repr, Inhabited for Node
-end Node
+namespace Err
+deriving instance Hashable, DecidableEq, Repr, Inhabited for Err
+
+@[always_inline]
+def str (msg : String) : Err :=
+  .other "" msg
+
+end Err
+
+abbrev Except (α : Type) := _root_.Except Err α
+
+@[always_inline]
+instance : Utils.Map.AsNat Var where
+  toNat := Var.idx
+  ofNat := Var.ofIdx
 
 /--
-An `Aig` with just the constant node.
+  An abstract representation of the mapping from variables to the corresponding node in the Aig.
+  This allows an abstract representation of variable validity (`var ∈ aig.nodes`),
+  lookup (`aig.nodes[var]`) and size (`aig.nodes.size`).
+
+  NOTE: This should not be used in computation, instead preferring `var.validIn aig`, `aig[var]`
+  and `aig.size`.
 -/
-@[inline]
-def empty : Aig :=
-  {
-    aig := .empty,
-    hconst := by grind [Std.Sat.AIG.empty]
-    _inputs := .empty,
-    _latches := .empty,
-  }
+@[always_inline]
+def nodes (aig : Aig) : Utils.Map Var Node :=
+  .mk
+    (valid := (·.idx < aig._nodes.size))
+    (map := fun var valid => aig._nodes[var.idx].toNode var)
+    (size := aig._nodes.size)
+
+@[always_inline]
+instance : Utils.Map.AsNat InputIdx where
+  toNat := InputIdx.idx
+  ofNat := InputIdx.ofIdx
 
 /--
-The number of nodes currently allocated in aig.
+  An abstract representation of the mapping from `InputIdx`s to the corresponding input in the Aig.
+  This allows an abstract representation of index validity (`idx ∈ aig.inputs`),
+  lookup (`aig.inputs[idx]`) and size (`aig.inputs.size`).
+
+  NOTE: This should not be used in computation, instead preferring `idx.validIn aig`,
+  `idx.getVar aig` and `aig.numInputs`.
+-/
+@[always_inline]
+def inputs (aig : Aig) : Utils.Map InputIdx Input :=
+  Utils.Map.ofPool aig._inputs InputIdx |>.mapVal (·.val)
+
+@[always_inline]
+instance : Utils.Map.AsNat LatchIdx where
+  toNat := LatchIdx.idx
+  ofNat := LatchIdx.ofIdx
+
+/--
+  An abstract representation of the mapping from `LatchIdx`s to the corresponding latch in the Aig.
+  This allows an abstract representation of index validity (`idx ∈ aig.latches`),
+  lookup (`aig.latches[idx]`) and size (`aig.latches.size`).
+
+  NOTE: This should not be used in computation, instead preferring `idx.validIn aig`,
+  `idx.getVar aig`/`idx.getNext aig`/`idx.getReset aig` and `aig.numLatches`.
+-/
+@[always_inline]
+def latches (aig : Aig) : Utils.Map LatchIdx Latch :=
+  Utils.Map.ofPool aig._latches LatchIdx |>.mapVal (·.val)
+
+/--
+  The number of nodes currently allocated in the Aig.
+  This includes both And gates as well as inputs and latches.
 -/
 @[always_inline]
 def size (aig : Aig) : Nat :=
-  aig.aig.decls.size
+  aig._nodes.size
 
 /--
-The maximum variable currently allocated in the aig.
--/
-@[always_inline]
-def maxVar (aig : Aig) : Var :=
-  .ofIdx <| aig.size - 1
-
-/--
-The number of input nodes in the aig.
+  The number of inputs in the Aig.
 -/
 @[always_inline]
 def numInputs (aig : Aig) : Nat :=
   aig._inputs.size
 
 /--
-The number of latch nodes in the aig.
+  The number of latches in the Aig.
 -/
 @[always_inline]
 def numLatches (aig : Aig) : Nat :=
   aig._latches.size
 
 /--
-The number of gate nodes in the aig.
+  The number of and gate nodes in the Aig.
 -/
-@[always_inline]
 abbrev numGates (aig : Aig) : Nat :=
   aig.size - aig.numInputs - aig.numLatches - 1
+
+/--
+  The variable with the highest index currently allocated in the Aig.
+  All variables up to this variable are also allocated.
+-/
+@[always_inline]
+def maxVar (aig : Aig) : Var :=
+  .ofIdx <| aig.size - 1
+
+/--
+  The smallest variable not currently allocated in the Aig.
+  This is the variable that is allocated for methods that append a node.
+-/
+@[always_inline]
+def nextVar (aig : Aig) : Var :=
+  .ofIdx <| aig.size
+
+@[simp, grind .]
+theorem not_constant_next_var :
+    aig.nextVar ≠ .constant := by
+  grind [nextVar, size, aig.sized]
+
+/--
+  The (arbitrary) next input index not currently allocated in the Aig.
+  This is the index that is allocated for methods that append an input.
+-/
+@[always_inline]
+def newInputIdx (aig : Aig) : InputIdx :=
+  .ofIdx aig._inputs.nextIdx
+
+/--
+  The (arbitrary) next latch index not currently allocated in the Aig.
+  This is the index that is allocated for methods that append a latch.
+-/
+@[always_inline]
+def newLatchIdx (aig : Aig) : LatchIdx :=
+  .ofIdx aig._latches.nextIdx
+
+/--
+  An Aig with just the constant node.
+-/
+def empty : Aig :=
+  {
+    _nodes := #[.false],
+    _inputs := .empty,
+    _latches := .empty,
+    sized := by grind
+  }
 
 end Aig
 
 /-
-Variable accessors.
+  Validity predicates.
 -/
 namespace Var 
 
+/--
+  A variable is `validIn` an Aig iff it has a node defined for it.
+-/
+@[expose]
 def validIn (var : Var) (aig : Aig) : Prop :=
   var.idx < aig.size
 
@@ -205,39 +391,28 @@ instance {var : Var} {aig : Aig} : Decidable (var.validIn aig) :=
     simp [Var.validIn]
   decidable_of_iff' _ this
 
+/--
+  A dependently type variable that is known to be valid in a given Aig.
+  This allows packing the proof of validity together with the variable.
+-/
 abbrev In (aig : Aig) := { var : Var // var.validIn aig }
 
+/--
+  Cast a `Var` into a `Var.In aig`. This tries to use `grind` to prove that the variable is
+  valid in the Aig.
+-/
 @[always_inline, simp]
 abbrev castIn (var : Var) (aig : Aig) (valid : var.validIn aig := by grind) : Var.In aig :=
   ⟨var, valid⟩
-
-private theorem validIn_iff_lt_decls_size {var : Var} :
-    var.validIn aig ↔ var.idx < aig.aig.decls.size := by
-  grind [validIn, Aig.size]
-
-grind_pattern validIn_iff_lt_decls_size => var.idx ≥ aig.aig.decls.size
-
-@[simp]
-private theorem lt_decls_size_of_validIn {var : Var} (valid : var.validIn aig) :
-    var.idx < aig.aig.decls.size :=
-  validIn_iff_lt_decls_size.mp valid
-
-theorem validIn_iff {var : Var} :
-    var.validIn aig ↔ var.idx < aig.size := by
-  grind [validIn]
-
-grind_pattern validIn_iff => var.idx ≥ aig.size
-
-@[simp]
-theorem lt_size_of_validIn {var : Var} (valid : var.validIn aig) :
-    var.idx < aig.size :=
-  validIn_iff.mp valid
 
 end Var
 
 namespace Lit
 
-@[expose, reducible, simp, grind unfold]
+/--
+  A literal is `validIn` an Aig iff its variable is also.
+-/
+@[always_inline, reducible, expose, simp, grind unfold]
 def validIn (lit : Lit) (aig : Aig) : Prop :=
   lit.var.validIn aig
 
@@ -246,8 +421,16 @@ instance {lit : Lit} {aig : Aig} : Decidable (lit.validIn aig) :=
   have : lit.validIn aig ↔ lit.var.validIn aig := by simp
   decidable_of_iff' _ this
 
+/--
+  A dependently type literal that is known to be valid in a given Aig.
+  This allows packing the proof of validity together with the literal.
+-/
 abbrev In (aig : Aig) := { lit : Lit // lit.validIn aig }
 
+/--
+  Cast a `Lit` into a `Lit.In aig`. This tries to use `grind` to prove that the literal is
+  valid in the Aig.
+-/
 @[always_inline, simp]
 abbrev castIn (lit : Lit) (aig : Aig) (valid : lit.validIn aig := by grind) : Lit.In aig :=
   ⟨lit, valid⟩
@@ -256,188 +439,250 @@ end Lit
 
 namespace Aig
 
-variable {aig : Aig}
-
-@[always_inline]
-def get (aig : Aig) (var : Var) (valid : var.validIn aig := by grind) : Node :=
-  match aig.aig.decls[var.idx] with
-  | .false => .false
-  | .atom (.input idx) => .input idx
-  | .atom (.latch idx) => .latch idx
-  | .gate rhs0 rhs1 => .and (.ofFanin rhs0) (.ofFanin rhs1)
-
-private theorem getElem_decls_eq_get {idx : Nat} (valid : idx < aig.aig.decls.size) :
-    aig.aig.decls[idx] =
-    match aig.get (Var.ofIdx idx) (by grind [Var.validIn, size]) with
-    | .false     => .false
-    | .input idx => .atom (.input idx)
-    | .latch idx => .atom (.latch idx)
-    | .and rhs0 rhs1 => .gate rhs0.toFanin rhs1.toFanin := by
-  grind [Aig.get]
-
-private theorem get_eq_getElem_decls {var : Var} (valid : var.validIn aig) :
-    aig.get var valid =
-    match aig.aig.decls[var.idx]'valid with
-    | .false     => .false
-    | .atom (.input idx) => .input idx
-    | .atom (.latch idx) => .latch idx
-    | .gate rhs0 rhs1 => .and (.ofFanin rhs0) (.ofFanin rhs1) := by
-  grind [Aig.get]
-
-private theorem get_eq_getElem_decls_false {var : Var} (valid : var.validIn aig)
-    (h : aig.get var valid = .false) :
-    aig.aig.decls[var.idx]'valid = .false := by
-  grind [get_eq_getElem_decls valid]
-
-private theorem get_eq_getElem_decls_input {var : Var} (valid : var.validIn aig)
-    {idx : InputIdx} (h : aig.get var valid = .input idx) :
-    aig.aig.decls[var.idx]'valid = .atom (.input idx) := by
-  grind [get_eq_getElem_decls valid]
-
-private theorem get_eq_getElem_decls_latch {var : Var} (valid : var.validIn aig)
-    {idx : LatchIdx} (h : aig.get var valid = .latch idx) :
-    aig.aig.decls[var.idx]'valid = .atom (.latch idx) := by
-  grind [get_eq_getElem_decls valid]
-
-private theorem get_eq_getElem_decls_and {var : Var} (valid : var.validIn aig)
-    {rhs0 rhs1 : Lit} (h : aig.get var valid = .and rhs0 rhs1) :
-    aig.aig.decls[var.idx]'valid = .gate rhs0.toFanin rhs1.toFanin := by
-  grind [get_eq_getElem_decls valid]
-
-@[always_inline, expose, reducible]
-instance instGetElemVar : GetElem Aig Var Node (fun aig var => var.validIn aig) where
-  getElem aig var (h := by grind) :=
-    aig.get var h
-
-@[simp, grind =]
-theorem getElem_eq_get {var : Var} (valid : var.validIn aig) :
-    aig[var]'valid = aig.get var valid := by
-  rfl
-
-@[simp, grind =]
-theorem getElem?_eq {var : Var} :
-    aig[var]? =
-    if h : var.validIn aig then
-      some aig[var]
-    else
-      none := by
-  split
-  · rw [getElem?_eq_some_getElem_iff]
-    trivial
-  · grind
-
-@[simp]
-theorem validIn_of_getElem?_some {var : Var} {node : Node} (h : aig[var]? = some node) :
-    var.validIn aig := by
-  grind
-
-grind_pattern validIn_of_getElem?_some => aig[var]?, some node, var.validIn aig
-
-/-
-Input accessors.
--/
 namespace InputIdx
 
+/--
+  An input is `validIn` an Aig iff it is a member of `aig.inputs`.
+-/
 @[local simp]
 def validIn (idx : InputIdx) (aig : Aig) : Prop :=
   idx.idx ∈ aig._inputs
 
+/-- NOTE: Do not rely on this function externally! -/
 @[always_inline]
 def instDecidableValidIn.impl (idx : InputIdx) (aig : Aig) : Bool :=
   idx.idx ∈ aig._inputs
 
 @[always_inline]
-instance {idx : InputIdx} {aig : Aig} : Decidable (idx.validIn aig) :=
+instance {idx : InputIdx} : Decidable (idx.validIn aig) :=
   have : idx.validIn aig ↔ instDecidableValidIn.impl idx aig := by
     simp [instDecidableValidIn.impl]
   decidable_of_iff' _ this
 
+/--
+  A dependently type `InputIdx` that is known to be valid in a given Aig.
+  This allows packing the proof of validity together with the index.
+-/
 abbrev In (aig : Aig) := { idx : InputIdx // idx.validIn aig }
 
+/--
+  Cast an `InputIdx` into an `InputIdx.In aig`. This tries to use `grind` to prove that the index is
+  valid in the Aig.
+-/
 @[always_inline, simp]
 abbrev castIn (idx : InputIdx) (aig : Aig) (valid : idx.validIn aig := by grind) : InputIdx.In aig :=
   ⟨idx, valid⟩
 
-@[always_inline]
-def getVar (idx : InputIdx) (aig : Aig) (valid : idx.validIn aig := by grind) : Var :=
-  aig._inputs[idx.idx].var
-
-@[always_inline, simp]
-abbrev getLit (idx : InputIdx) (aig : Aig) (valid : idx.validIn aig := by grind) : Lit :=
-  idx.getVar aig valid |>.toLit
-
 end InputIdx
 
-/-
-Latch accessors.
--/
 namespace LatchIdx
 
+/--
+  A latch is `validIn` an Aig iff it is a member of `aig.latches`.
+-/
 @[local simp]
 def validIn (idx : LatchIdx) (aig : Aig) : Prop :=
   idx.idx ∈ aig._latches
 
+/-- NOTE: Do not rely on this function externally! -/
 @[always_inline]
 def instDecidableValidIn.impl (idx : LatchIdx) (aig : Aig) : Bool :=
   idx.idx ∈ aig._latches
 
 @[always_inline]
-instance {idx : LatchIdx} {aig : Aig} : Decidable (idx.validIn aig) :=
+instance {idx : LatchIdx} : Decidable (idx.validIn aig) :=
   have : idx.validIn aig ↔ instDecidableValidIn.impl idx aig := by
     simp [instDecidableValidIn.impl]
   decidable_of_iff' _ this
 
+/--
+  A dependently type `LatchIdx` that is known to be valid in a given Aig.
+  This allows packing the proof of validity together with the index.
+-/
 abbrev In (aig : Aig) := { idx : LatchIdx // idx.validIn aig }
 
+/--
+  Cast an `LatchIdx` into an `LatchIdx.In aig`. This tries to use `grind` to prove that the index is
+  valid in the Aig.
+-/
 @[always_inline, simp]
 abbrev castIn (idx : LatchIdx) (aig : Aig) (valid : idx.validIn aig := by grind) : LatchIdx.In aig :=
   ⟨idx, valid⟩
 
-@[always_inline]
-def getVar (idx : LatchIdx) (aig : Aig) (valid : idx.validIn aig := by grind) : Var :=
-  aig._latches[idx.idx].var
+end LatchIdx
 
-@[always_inline, simp]
-abbrev getLit (idx : LatchIdx) (aig : Aig) (valid : idx.validIn aig := by grind) : Lit :=
+/-- NOTE: Do not rely on this function externally! -/
+@[always_inline]
+def instGetElemVar.impl (aig : Aig) (var : Var) (valid : var.validIn aig := by grind) : Node :=
+  aig._nodes[var.idx].toNode var
+
+@[always_inline]
+instance instGetElemVar : GetElem Aig Var Node (fun aig var => var.validIn aig) where
+  getElem aig var (h := by grind) :=
+    instGetElemVar.impl aig var h
+
+/-
+  Input accessors.
+-/
+namespace InputIdx
+
+/--
+  Lookup the variable (PI) defined by this input in the Aig.
+-/
+@[inline]
+def getVar (idx : InputIdx) (aig : Aig) (valid : idx.validIn aig := by grind) : Var :=
+  aig._inputs[idx.idx].val.var
+
+/--
+  Lookup the variable (PI) defined by this input in the Aig.
+
+  If `idx` isn't valid in the Aig, throws `err`.
+-/
+@[always_inline]
+def getVar! (idx : InputIdx) (aig : Aig) (err : Err := .invalidIdx "InputIdx.getVar!" "idx") : Except Var :=
+  match aig._inputs[idx.idx]? with
+  | some input => return input.val.var
+  | none       => throw err
+
+/--
+  Lookup the variable defined by this input in the Aig and cast it to an uninverted literal.
+-/
+@[inline]
+def getLit (idx : InputIdx) (aig : Aig) (valid : idx.validIn aig := by grind) : Lit :=
   idx.getVar aig valid |>.toLit
 
+/--
+  Lookup the variable defined by this input in the Aig and cast it to an uninverted literal.
+
+  If `idx` isn't valid in the Aig, throws `err`.
+-/
 @[always_inline]
+def getLit! (idx : InputIdx) (aig : Aig) (err : Err := .invalidIdx "InputIdx.getLit!" "idx") : Except Lit :=
+  match aig._inputs[idx.idx]? with
+  | some input => return input.val.var.toLit
+  | none       => throw err
+
+end InputIdx
+
+/-
+  Latch accessors.
+-/
+namespace LatchIdx
+
+/--
+  Lookup the variable (CI) defined by this latch in the Aig.
+-/
+@[inline]
+def getVar (idx : LatchIdx) (aig : Aig) (valid : idx.validIn aig := by grind) : Var :=
+  aig._latches[idx.idx].val.var
+
+/--
+  Lookup the variable (CI) defined by this latch in the Aig.
+
+  If `idx` isn't valid in the Aig, throws `err`.
+-/
+@[always_inline]
+def getVar! (idx : LatchIdx) (aig : Aig) (err : Err := .invalidIdx "LatchIdx.getVar!" "idx") : Except Var :=
+  match aig._latches[idx.idx]? with
+  | some latch => return latch.val.var
+  | none       => throw err
+
+/--
+  Lookup the variable defined by this latch in the Aig and cast it to an uninverted literal.
+-/
+@[inline]
+def getLit (idx : LatchIdx) (aig : Aig) (valid : idx.validIn aig := by grind) : Lit :=
+  idx.getVar aig valid |>.toLit
+
+/--
+  Lookup the variable defined by this latch in the Aig and cast it to an uninverted literal.
+
+  If `idx` isn't valid in the Aig, throws `err`.
+-/
+@[always_inline]
+def getLit! (idx : LatchIdx) (aig : Aig) (err : Err := .invalidIdx "LatchIdx.getLit!" "idx") : Except Lit :=
+  match aig._latches[idx.idx]? with
+  | some latch => return latch.val.var.toLit
+  | none       => throw err
+
+/--
+  Lookup the next state function defined for this latch in the Aig.
+-/
+@[inline]
 def getNext (idx : LatchIdx) (aig : Aig) (valid : idx.validIn aig := by grind) : Lit :=
-  aig._latches[idx.idx].next
+  aig._latches[idx.idx].val.next
 
-@[always_inline]
-def setNext (idx : LatchIdx) (aig : Aig) (next : Lit) : Aig :=
-  { aig with _latches := aig._latches.modify idx.idx ({ · with next }) }
+/--
+  Lookup the next state function defined for this latch in the Aig.
 
+  If `idx` isn't valid in the Aig, throws `err`.
+-/
 @[always_inline]
+def getNext! (idx : LatchIdx) (aig : Aig) (err : Err := .invalidIdx "LatchIdx.getNext!" "idx") : Except Lit :=
+  match aig._latches[idx.idx]? with
+  | some latch => return latch.val.next
+  | none       => throw err
+
+/--
+  Lookup the optional reset function defined for this latch in the Aig.
+-/
+@[inline]
 def getReset (idx : LatchIdx) (aig : Aig) (valid : idx.validIn aig := by grind) : Option Lit :=
-  aig._latches[idx.idx].reset
+  aig._latches[idx.idx].val.reset
 
+/--
+  Lookup the optional reset function defined for this latch in the Aig.
+
+  If `idx` isn't valid in the Aig, throws `err`.
+-/
 @[always_inline]
-def setReset (idx : LatchIdx) (aig : Aig) (reset : Option Lit) : Aig :=
-  { aig with _latches := aig._latches.modify idx.idx ({ · with reset }) }
+def getReset! (idx : LatchIdx) (aig : Aig) (err : Err := .invalidIdx "LatchIdx.getReset!" "idx") : Except (Option Lit) :=
+  match aig._latches[idx.idx]? with
+  | some latch => return latch.val.reset
+  | none       => throw err
+
+set_option linter.unusedVariables false in
+/--
+  Update the next state function for a latch in the Aig.
+-/
+@[inline]
+def setNext (idx : LatchIdx) (aig : Aig) (next : Lit) (valid : idx.validIn aig := by grind) : Aig :=
+  { aig with _latches := aig._latches.modify idx.idx (⟨{ ·.val with next }, by grind⟩) }
+
+/--
+  Update the next state function for a latch in the Aig.
+
+  If `idx` isn't valid in the Aig, throws `err`.
+-/
+@[always_inline]
+def setNext! (idx : LatchIdx) (aig : Aig) (next : Lit) (err : Err := .invalidIdx "LatchIdx.setNext!" "idx") : Except Aig :=
+  if _ : idx.validIn aig then
+    return idx.setNext aig next
+  else
+    throw err
+
+set_option linter.unusedVariables false in
+/--
+  Update the reset function for a latch in the Aig.
+-/
+@[inline]
+def setReset (idx : LatchIdx) (aig : Aig) (reset : Option Lit) (valid : idx.validIn aig := by grind) : Aig :=
+  { aig with _latches := aig._latches.modify idx.idx (⟨{ ·.val with reset }, by grind⟩) }
+
+/--
+  Update the reset function for a latch in the Aig.
+
+  If `idx` isn't valid in the Aig, throws `err`.
+-/
+@[always_inline]
+def setReset! (idx : LatchIdx) (aig : Aig) (reset : Option Lit) (err : Err := .invalidIdx "LatchIdx.setReset!" "idx") : Except Aig :=
+  if _ : idx.validIn aig then
+    return idx.setReset aig reset
+  else
+    throw err
 
 end LatchIdx
 
-theorem numInputs_zero_iff_not_validIn :
-    aig.numInputs = 0 ↔ ∀ (idx : InputIdx), ¬idx.validIn aig := by
-  simp [InputIdx.validIn, numInputs, Utils.Pool.size_zero_iff_forall_not_in]
-  constructor
-  · grind
-  · intro h
-    grind [h (.ofIdx _)]
-
-theorem numLatches_zero_iff_not_validIn :
-    aig.numLatches = 0 ↔ ∀ (idx : LatchIdx), ¬idx.validIn aig := by
-  simp [LatchIdx.validIn, numLatches, Utils.Pool.size_zero_iff_forall_not_in]
-  constructor
-  · grind
-  · intro h
-    grind [h (.ofIdx _)]
-
-/-
-Arbitrary index validity and accessors, defined as abbreviations
--/
 namespace LeafIdx
 
 @[inline]
@@ -445,61 +690,29 @@ def asInput (idx : LeafIdx) (h : idx matches .input _ := by grind) : InputIdx :=
   match idx, h with
   | .input idx, _ => idx
 
-@[simp, grind =]
-theorem asInput_of_input {idx : InputIdx} :
-    (input idx).asInput = idx := by
-  rfl
-
 @[inline]
 def asLatch (idx : LeafIdx) (h : idx matches .latch _ := by grind) : LatchIdx :=
   match idx, h with
   | .latch idx, _ => idx
 
-@[simp, grind =]
-theorem asLatch_of_latch {idx : LatchIdx} :
-    (latch idx).asLatch = idx := by
-  rfl
-
+@[local grind]
 def validIn (idx : LeafIdx) (aig : Aig) : Prop :=
   match idx with
-  | .input idx => idx.validIn aig
+  | .input idx
   | .latch idx => idx.validIn aig
 
-@[simp]
-theorem validIn_iff {idx : LeafIdx} :
-    idx.validIn aig ↔
-    match idx with
-    | .input idx => idx.validIn aig
-    | .latch idx => idx.validIn aig := by
-  grind [validIn]
-
--- Only unfold with this pattern when not trivially an input or latch
-grind_pattern validIn_iff => idx.validIn aig where
-  idx =/= .input _
-  idx =/= .latch _
-
-@[grind =]
-theorem validIn_input {idx : InputIdx} :
-    (input idx).validIn aig ↔ idx.validIn aig := by
-  grind [validIn]
-
-@[grind =]
-theorem validIn_latch {idx : LatchIdx} :
-    (latch idx).validIn aig ↔ idx.validIn aig := by
-  grind [validIn]
-
 instance {idx : InputIdx} : Coe (idx.validIn aig) ((idx : LeafIdx).validIn aig) where
-  coe := by grind
+  coe := by grind [validIn]
 
 instance {idx : LatchIdx} : Coe (idx.validIn aig) ((idx : LeafIdx).validIn aig) where
-  coe := by grind
+  coe := by grind [validIn]
 
 @[always_inline]
-instance {idx : LeafIdx} {aig : Aig} : Decidable (idx.validIn aig) := by
-  rw [validIn_iff]
-  match idx with
-  | .input idx => infer_instance
-  | .latch idx => infer_instance
+instance {idx : LeafIdx} {aig : Aig} : Decidable (idx.validIn aig) :=
+  match h : idx with
+  | .input idx
+  | .latch idx =>
+    decidable_of_bool (idx.validIn aig) (by grind)
 
 abbrev In (aig : Aig) := { idx : LeafIdx // idx.validIn aig }
 
@@ -515,153 +728,404 @@ instance : Coe (InputIdx.In aig) (LeafIdx.In aig) where
 instance : Coe (LatchIdx.In aig) (LeafIdx.In aig) where
   coe idx := ⟨idx, idx.property⟩
 
+/--
+  Lookup the variable(CI) defined by this leaf in the Aig.
+-/
 @[always_inline]
 def getVar (idx : LeafIdx) (aig : Aig) (valid : idx.validIn aig := by grind) : Var :=
   match idx with
-  | .input idx => idx.getVar aig
+  | .input idx
   | .latch idx => idx.getVar aig
 
-@[simp]
-theorem getVar_def {idx : LeafIdx} (valid : idx.validIn aig) :
-    idx.getVar aig valid =
-    match idx with
-    | .input idx => idx.getVar aig
-    | .latch idx => idx.getVar aig := by
-  grind [getVar]
+/--
+  Lookup the variable (CI) defined by this leaf in the Aig.
 
-grind_pattern getVar_def => idx.getVar aig where
-  idx =/= .input _
-  idx =/= .latch _
+  If `idx` isn't valid in the Aig, throws `err`.
+-/
+@[always_inline]
+def getVar! (idx : LeafIdx) (aig : Aig) (err : Err := .invalidIdx "LeafIdx.getVar!" "idx") : Except Var :=
+  match idx with
+  | .input idx
+  | .latch idx => idx.getVar! aig err
 
-@[simp, grind =]
-theorem getVar_input {idx : InputIdx} (valid : (input idx).validIn aig) :
-    (input idx).getVar aig = idx.getVar aig := by
-  grind [getVar]
-
-@[simp, grind =]
-theorem getVar_latch {idx : LatchIdx} (valid : (latch idx).validIn aig) :
-    (latch idx).getVar aig = idx.getVar aig := by
-  grind [getVar]
-
-@[always_inline, expose, simp, grind unfold]
+/--
+  Lookup the variable (CI) defined by this leaf in the Aig and cast it to an uninverted literal.
+-/
+@[always_inline]
 def getLit (idx : LeafIdx) (aig : Aig) (valid : idx.validIn aig := by grind) : Lit :=
   idx.getVar aig valid |>.toLit
+
+/--
+  Lookup the variable (CI) defined by this leaf in the Aig and cast it to an uninverted literal.
+
+  If `idx` isn't valid in the Aig, throws `err`.
+-/
+@[always_inline]
+def getLit! (idx : LeafIdx) (aig : Aig) (err : Err := .invalidIdx "LeafIdx.getLit!" "idx") : Except Lit :=
+  match idx with
+  | .input idx
+  | .latch idx => idx.getLit! aig err
 
 end LeafIdx
 
 /--
-Appends an input to the Aig with the given index. This is normally of use when this index is
-provably not in the Aig (for example when the Aig is empty) and it already carries meaning in
-another Aig.
-
-If another input is already registered for this index, this will overwrite it which can break
-well-formedness.
+  Push a new node onto the `Aig` from its data. This has the variable `aig.nextVar`.
 -/
-@[inline]
-def addInput' (aig : Aig) (idx : InputIdx) : Aig :=
-  -- Construct an atom pointing to this index
-  let res := aig.aig.mkAtom <| .input idx
-
-  -- Build input metadata pointing to this new atom and update the index in the pool to this
-  let _inputs := aig._inputs.insert idx.idx { var := .ofRef res.ref }
-
-  have hconst := by grind [aig.aig.hzero, aig.hconst, Std.mkAtom_eq_decls_push]
-  { aig with aig := res.aig, hconst, _inputs }
+@[always_inline]
+private def pushNode (aig : Aig) (node : NodeData) : Aig :=
+  { aig with _nodes := aig._nodes.push node, sized := by grind }
 
 /--
-Appends an input with a fresh index to the Aig, returning the index of the input.
+  Overwrite a node at a given index in the `Aig`.
+  TODO: This currently breaks linearity, so the existing node data is dealloced and
+  a new node alloced.
 -/
-@[inline]
+@[always_inline]
+private def setNode (aig : Aig) (var : Var) (node : NodeData) (valid : var.validIn aig := by grind) : Aig :=
+  { aig with _nodes := aig._nodes.set var.idx node, sized := by grind [aig.sized] }
+
+@[always_inline]
+private def insertInput (aig : Aig) (idx : InputIdx) (input : Input) (h : input.var ≠ .constant := by grind) : Aig :=
+  { aig with _inputs := aig._inputs.insert idx.idx ⟨input, h⟩ }
+
+@[always_inline]
+private def insertLatch (aig : Aig) (idx : LatchIdx) (latch : Latch) (h : latch.var ≠ .constant := by grind) : Aig :=
+  { aig with _latches := aig._latches.insert idx.idx ⟨latch, h⟩ }
+
+@[always_inline]
+private def eraseInput (aig : Aig) (idx : InputIdx) : Aig :=
+  { aig with _inputs := aig._inputs.erase idx.idx }
+
+@[always_inline]
+private def eraseLatch (aig : Aig) (idx : LatchIdx) : Aig :=
+  { aig with _latches := aig._latches.erase idx.idx }
+
+attribute [local grind] InputIdx.validIn LatchIdx.validIn newInputIdx newLatchIdx
+
+set_option linter.unusedVariables false in
+/--
+  Append an input with a new index to the Aig, returning the index of the input.
+-/
+@[always_inline]
 def addInput (aig : Aig) : Aig × InputIdx :=
-  -- Add a new input at the next free index, and return the index
-  let idx := .ofIdx aig._inputs.nextIdx
-  (aig.addInput' idx, idx)
-
-theorem addInput_eq :
-    aig.addInput = (aig.addInput' (aig.addInput.snd), aig.addInput.snd) := by
-  simp [addInput]
-
-@[simp, grind =]
-theorem addInput_fst_eq :
-    aig.addInput.fst = aig.addInput' (aig.addInput.snd) := by
-  rw [addInput_eq]
+  let idx := aig.newInputIdx
+  let var := aig.nextVar
+  let aig := aig.pushNode <| .input idx var
+  let aig := aig.insertInput idx { var }
+  (aig, idx)
 
 /--
-Appends an latch to the Aig with the given index. This is normally of use when this index is
-provably not in the Aig (for example when the Aig is empty) and it already carries meaning in
-another Aig.
+  Append a latch with a new index to the Aig, returning the index of the latch.
 
-If another latch is already registered for this index, this will overwrite it which can break
-well-formedness.
+  If `next` and `reset` are not known yet, they should be set to placeholders
+  (like `Lit.false`/`Option.none`) and updated later with `LatchIdx.setNext`/`LatchIdx.setReset`.
 -/
-@[inline]
-def addLatch' (aig : Aig) (idx : LatchIdx) (next : Lit) (reset : Option Lit) : Aig :=
-  -- Construct an atom pointing to this index
-  let res := aig.aig.mkAtom <| .latch idx
-
-  -- Build latch metadata pointing to this new atom and update the index in the pool to this
-  let latch := { var := .ofRef res.ref, next, reset }
-  let _latches := aig._latches.insert idx.idx latch
-
-  have hconst := by grind [aig.aig.hzero, aig.hconst, Std.mkAtom_eq_decls_push]
-  { aig with aig := res.aig, hconst, _latches }
+@[always_inline]
+def addLatch (aig : Aig) (next : Lit) (reset : Option Lit := none) : Aig × LatchIdx :=
+  let idx := aig.newLatchIdx
+  let var := aig.nextVar
+  let aig := aig.pushNode <| .latch idx var
+  let aig := aig.insertLatch idx { var, next, reset }
+  (aig, idx)
 
 /--
-Appends a latch with a fresh index to the Aig, returning the index of the input. The next and
-reset values are set appropriately. If they are not available yet at construction time, they
-should be set to placeholders (like `Lit.false`) and updated later with `setNext`/`setReset`.
+  Append an and gate to the Aig, returning the variable defined by the new gate.
+  This does not perform any optimizations.
+
+  Note that neither input shuld be set to `nextVar` (equivalent to `Var.ofIdx aig.size`)
+  or internal invariants are broken.
 -/
-@[inline]
-def addLatch (aig : Aig) (next : Lit) (reset : Option Lit) : Aig × LatchIdx :=
-  -- Add a new latch at the next free index, and return the index
-  let idx := .ofIdx aig._latches.nextIdx
-  (aig.addLatch' idx next reset, idx)
-
-theorem addLatch_eq {next : Lit} {reset : Option Lit} :
-    aig.addLatch next reset =
-    (aig.addLatch' (aig.addLatch next reset |>.snd) next reset, aig.addLatch next reset |>.snd) := by
-  simp [addLatch]
-
-@[simp, grind =]
-theorem addLatch_fst_eq {next : Lit} {reset : Option Lit} :
-    (aig.addLatch next reset).fst = aig.addLatch' (aig.addLatch next reset |>.snd) next reset := by
-  rw [addLatch_eq]
+@[always_inline]
+def addAnd (aig : Aig) (rhs0 rhs1 : Lit) : Aig × Var :=
+  let var := aig.nextVar
+  let aig := aig.pushNode <| .and rhs0 rhs1
+  (aig, var)
 
 /--
-Appends a new and gate to the Aig, applying structural hashing to exploit reuse.
+  Convert an input into a new latch that defines the same variable, deleting the input.
+-/
+def InputIdx.convertToLatch (idx : InputIdx) (aig : Aig) (next : Lit) (reset : Option Lit := none)
+    (valid : idx.validIn aig := by grind)
+    (varValid : (idx.getVar aig).validIn aig := by grind) : Aig × LatchIdx :=
+  let var := idx.getVar aig
+  let latch := aig.newLatchIdx
+  let aig := aig.setNode var <| .latch latch var
+  let aig := aig.eraseInput idx
+  let aig := aig.insertLatch latch { var, next, reset } (by grind [getVar])
+  (aig, latch)
 
-TODO: Currently this requires proofs that rhs0/rhs1 are valid in the aig, but after switching to
-buffed (and getting rid of dependent typing) this won't be needed anymore
+/--
+  Convert an input into a new latch that defines the same variable, deleting the input.
+
+  If `idx` is not valid in `aig`, throws `errInvalid`.
+  Otherwise if `idx.getVar aig` is not valid in `aig`, throws `errVarInvalid`.
+-/
+@[always_inline]
+def InputIdx.convertToLatch! (idx : InputIdx) (aig : Aig) (next : Lit) (reset : Option Lit := none)
+    (errInvalid    : Err := .invalidIdx "InputIdx.convertToLatch!" "idx")
+    (errVarInvalid : Err := .invalidIdx "InputIdx.convertToLatch!" "idx.getVar aig") : Except (Aig × LatchIdx) :=
+  if _ : ¬idx.validIn aig then
+    throw errInvalid
+  else if _ : ¬(idx.getVar aig).validIn aig then
+    throw errVarInvalid
+  else
+    return idx.convertToLatch aig next reset
+
+/--
+  Convert an input into a new and gate that defines the same variable, deleting the input.
 -/
 @[inline]
-def addAnd (aig : Aig) (rhs0 rhs1 : Lit)
-    (valid0 : rhs0.validIn aig := by grind) (valid1 : rhs1.validIn aig := by grind) : Aig × Lit :=
-  let res := aig.aig.mkAndCached ⟨rhs0.toRef valid0, rhs1.toRef valid1⟩
-  have hconst := by
-    intro i
-    by_cases i ≥ aig.aig.decls.size
-    <;> grind [aig.aig.hzero, aig.hconst, aig.aig.mkAndCached_decl_eq, Std.mkAndCached_matches_gate (aig := aig.aig)]
-  let aig := { aig with aig := res.aig, hconst }
-  (aig, .ofRef res.ref)
+def InputIdx.convertToAnd (idx : InputIdx) (aig : Aig) (rhs0 rhs1 : Lit)
+    (valid : idx.validIn aig := by grind)
+    (varValid : (idx.getVar aig).validIn aig := by grind) : Aig :=
+  let var := idx.getVar aig
+  let aig := aig.setNode var <| .and rhs0 rhs1
+  let aig := aig.eraseInput idx
+  aig
 
-/-
-Setup get/set definitions for use locally as grind/simp rules, with grind_def/
-simp_def tactics to make use of them.
+/--
+  Convert an input into a new and gate that defines the same variable, deleting the input.
+
+  If `idx` is not valid in `aig`, throws `errInvalid`.
+  Otherwise if `idx.getVar aig` is not valid in `aig`, throws `errVarInvalid`.
 -/
-attribute [simp_valaig_defs, grind_valaig_defs]
-  Aig.get Aig.instGetElemVar Aig.size
-  Aig.empty
-  InputIdx.getVar
-  LatchIdx.getVar LatchIdx.getNext LatchIdx.getReset
-  LatchIdx.setNext LatchIdx.setReset
-  Aig.addInput Aig.addInput'
-  Aig.addLatch Aig.addLatch'
-  Aig.addAnd
+@[always_inline]
+def InputIdx.convertToAnd! (idx : InputIdx) (aig : Aig) (rhs0 rhs1 : Lit)
+    (errInvalid    : Err := .invalidIdx "InputIdx.convertToAnd!" "idx")
+    (errVarInvalid : Err := .invalidIdx "InputIdx.convertToAnd!" "idx.getVar aig") : Except Aig :=
+  if _ : ¬idx.validIn aig then
+    throw errInvalid
+  else if _ : ¬(idx.getVar aig).validIn aig then
+    throw errVarInvalid
+  else
+    return idx.convertToAnd aig rhs0 rhs1
 
-attribute [grind_valaig_defs] InputIdx LatchIdx
+set_option linter.unusedVariables false in
+/--
+  Change the input index used to define an input to a new known unused one.
+  This is mainly useful when trying to build a new Aig while preserving indices from an existing one.
+-/
+@[inline]
+def InputIdx.changeIdx (old new : InputIdx) (aig : Aig)
+    (valid : old.validIn aig := by grind)
+    (varValid : (old.getVar aig).validIn aig := by grind)
+    (unused : ¬new.validIn aig ∨ old = new := by grind) : Aig :=
+  let data := aig._inputs[old.idx]
+  let var := data.val.var
+  let aig := aig.setNode data.val.var (.input new data.val.var) (by grind [getVar])
+  let aig := aig.eraseInput old
+  let aig := aig.insertInput new data
+  aig
 
-attribute [simp_valaig_defs, grind_valaig_defs =]
-  Std.mkAtom_eq_decls_push Std.mkAtom_size Std.mkAtom_ref_eq_decls_size
-  Std.Sat.AIG.mkAndCached_decl_eq
+/--
+  Change the input index used to define an input to a new known unused one.
+  This is mainly useful when trying to build a new Aig while preserving indices from an existing one.
 
-attribute [grind_valaig_defs! .] Std.Sat.AIG.mkAndCached_le_size
+  If `old` is not valid in `aig`, throws `errInvalid`.
+  Otherwise if `old.getVar aig` is not valid in `aig`, throws `errVarInvalid`.
+  Otherwise if `new` is already valid in `aig` and not equal to `old`, throws `errUsed`.
+-/
+@[inline]
+def InputIdx.changeIdx! (old new : InputIdx) (aig : Aig)
+    (errInvalid    : Err := .invalidIdx "InputIdx.changeIdx!" "old")
+    (errVarInvalid : Err := .invalidIdx "InputIdx.changeIdx!" "old.getVar aig")
+    (errUsed       : Err := .other      "InputIdx.changeIdx!" "index new is already used") : Except Aig :=
+  if _ : ¬old.validIn aig then
+    throw errInvalid
+  else if _ : ¬(old.getVar aig).validIn aig then
+    throw errVarInvalid
+  else if _ : new ≠ old ∧ new.validIn aig then
+    throw errUsed
+  else
+    return old.changeIdx new aig
+
+/--
+  Convert a latch into a new input that defines the same variable, deleting the latch.
+-/
+def LatchIdx.convertToInput (idx : LatchIdx) (aig : Aig)
+    (valid : idx.validIn aig := by grind)
+    (varValid : (idx.getVar aig).validIn aig := by grind) : Aig × InputIdx :=
+  let var := idx.getVar aig
+  let input := aig.newInputIdx
+  let aig := aig.setNode var <| .input input var
+  let aig := aig.eraseLatch idx
+  let aig := aig.insertInput input { var } (by grind [getVar])
+  (aig, input)
+
+/--
+  Convert a latch into a new input that defines the same variable, deleting the latch.
+
+  If `idx` is not valid in `aig`, throws `errInvalid`.
+  Otherwise if `idx.getVar aig` is not valid in `aig`, throws `errVarInvalid`.
+-/
+@[always_inline]
+def LatchIdx.convertToInput! (idx : LatchIdx) (aig : Aig)
+    (errInvalid    : Err := .invalidIdx "LatchIdx.convertToInput!" "idx")
+    (errVarInvalid : Err := .invalidIdx "LatchIdx.convertToInput!" "idx.getVar aig") : Except (Aig × InputIdx) :=
+  if _ : ¬idx.validIn aig then
+    throw errInvalid
+  else if _ : ¬(idx.getVar aig).validIn aig then
+    throw errVarInvalid
+  else
+    return idx.convertToInput aig
+
+/--
+  Convert a latch into a new and gate that defines the same variable, deleting the latch.
+-/
+@[inline]
+def LatchIdx.convertToAnd (idx : LatchIdx) (aig : Aig) (rhs0 rhs1 : Lit)
+    (valid : idx.validIn aig := by grind)
+    (varValid : (idx.getVar aig).validIn aig := by grind) : Aig :=
+  let var := idx.getVar aig
+  let aig := aig.setNode var <| .and rhs0 rhs1
+  let aig := aig.eraseLatch idx
+  aig
+
+/--
+  Convert a latch into a new and gate that defines the same variable, deleting the latch.
+
+  If `idx` is not valid in `aig`, throws `errInvalid`.
+  Otherwise if `idx.getVar aig` is not valid in `aig`, throws `errVarInvalid`.
+-/
+@[always_inline]
+def LatchIdx.convertToAnd! (idx : LatchIdx) (aig : Aig) (rhs0 rhs1 : Lit)
+    (errInvalid    : Err := .invalidIdx "LatchIdx.convertToAnd!" "idx")
+    (errVarInvalid : Err := .invalidIdx "LatchIdx.convertToAnd!" "idx.getVar aig") : Except Aig :=
+  if _ : ¬idx.validIn aig then
+    throw errInvalid
+  else if _ : ¬(idx.getVar aig).validIn aig then
+    throw errVarInvalid
+  else
+    return idx.convertToAnd aig rhs0 rhs1
+
+set_option linter.unusedVariables false in
+/--
+  Change the latch index used to define a latch to a new known unused one.
+  This is mainly useful when trying to build a new Aig while preserving indices from an existing one.
+-/
+@[inline]
+def LatchIdx.changeIdx (old new : LatchIdx) (aig : Aig)
+    (valid : old.validIn aig := by grind)
+    (varValid : (old.getVar aig).validIn aig := by grind)
+    (unused : ¬new.validIn aig ∨ old = new := by grind) : Aig :=
+  let data := aig._latches[old.idx]
+  let var := data.val.var
+  let aig := aig.setNode data.val.var (.latch new data.val.var) (by grind [getVar])
+  let aig := aig.eraseLatch old
+  let aig := aig.insertLatch new data
+  aig
+
+/--
+  Change the latch index used to define a latch to a new known unused one.
+  This is mainly useful when trying to build a new Aig while preserving indices from an existing one.
+
+  If `old` is not valid in `aig`, throws `errInvalid`.
+  Otherwise if `old.getVar aig` is not valid in `aig`, throws `errVarInvalid`.
+  Otherwise if `new` is already valid in `aig` and not equal to `old`, throws `errUsed`.
+-/
+@[always_inline]
+def LatchIdx.changeIdx! (old new : LatchIdx) (aig : Aig)
+    (errInvalid    : Err := .invalidIdx "LatchIdx.changeIdx!" "old")
+    (errVarInvalid : Err := .invalidIdx "LatchIdx.changeIdx!" "old.getVar aig")
+    (errUsed       : Err := .other      "LatchIdx.changeIdx!" "index new is already used") : Except Aig :=
+  if _ : ¬old.validIn aig then
+    throw errInvalid
+  else if _ : ¬(old.getVar aig).validIn aig then
+    throw errVarInvalid
+  else if _ : new ≠ old ∧ new.validIn aig then
+    throw errUsed
+  else
+    return old.changeIdx new aig
+
+set_option linter.unusedVariables false in
+/--
+  Convert an and gate to a new input.
+-/
+@[inline]
+def convertAndToInput (aig : Aig) (var : Var)
+    (valid : var.validIn aig := by grind)
+    (isAnd : aig[var] matches .and _ _ := by grind) : Aig × InputIdx :=
+  let idx := aig.newInputIdx
+  let aig := aig.setNode var <| .input idx var
+  let aig := aig.insertInput idx { var }
+    (by simp only [instGetElemVar, instGetElemVar.impl, NodeData.toNode] at isAnd; grind)
+  (aig, idx)
+
+/--
+  Convert an and gate to a new input.
+
+  If `var` is not valid in `aig`, throws `errInvalid`.
+  Otherwise if `var` does not define an and gate, throws `errIsAnd`.
+-/
+@[always_inline]
+def convertAndToInput! (aig : Aig) (var : Var)
+    (errInvalid : Err := .invalidIdx "convertAndToInput!" "var")
+    (errIsAnd   : Err := .other      "convertAndToInput!" "expected existing node to be an and gate") : Except (Aig × InputIdx) :=
+  if _ : ¬var.validIn aig then
+    throw errInvalid
+  else if _ : ¬aig[var] matches .and _ _ then
+    throw errIsAnd
+  else
+    return aig.convertAndToInput var
+
+set_option linter.unusedVariables false in
+/--
+  Convert an and gate to a new latch.
+-/
+def convertAndToLatch (aig : Aig) (var : Var) (next : Lit) (reset : Option Lit := none)
+    (valid : var.validIn aig := by grind)
+    (isAnd : aig[var] matches .and _ _ := by grind) : Aig × LatchIdx :=
+  let idx := aig.newLatchIdx
+  let aig := aig.setNode var <| .latch idx var
+  let aig := aig.insertLatch idx { var, next, reset }
+    (by simp only [instGetElemVar, instGetElemVar.impl, NodeData.toNode] at isAnd; grind)
+  (aig, idx)
+
+/--
+  Convert an and gate to a new latch.
+
+  If `var` is not valid in `aig`, throws `errInvalid`.
+  Otherwise if `var` does not define an and gate, throws `errIsAnd`.
+-/
+@[always_inline]
+def convertAndToLatch! (aig : Aig) (var : Var) (next : Lit) (reset : Option Lit := none)
+    (errInvalid : Err := .invalidIdx "convertAndToLatch!" "var")
+    (errIsAnd   : Err := .other      "convertAndToLatch!" "expected existing node to be an and gate") : Except (Aig × LatchIdx) :=
+  if _ : ¬var.validIn aig then
+    throw errInvalid
+  else if _ : ¬aig[var] matches .and _ _ then
+    throw errIsAnd
+  else
+    return aig.convertAndToLatch var next reset
+
+set_option linter.unusedVariables false in
+/--
+  Update the arguments to an existing and gate.
+-/
+@[inline]
+def rewriteAnd (aig : Aig) (var : Var) (rhs0 rhs1 : Lit)
+    (valid : var.validIn aig := by grind)
+    (isAnd : aig[var] matches .and _ _ := by grind) : Aig :=
+  aig.setNode var (.and rhs0 rhs1)
+
+/--
+  Update the arguments to an existing and gate.
+
+  If `var` is not valid in `aig`, throws `errInvalid`.
+  Otherwise if `var` does not define an and gate, throws `errIsAnd`.
+-/
+@[always_inline]
+def rewriteAnd! (aig : Aig) (var : Var) (rhs0 rhs1 : Lit)
+    (errInvalid : Err := .invalidIdx "rewriteAnd!" "var")
+    (errIsAnd   : Err := .other      "rewriteAnd!" "expected existing node to be an and gate") : Except Aig :=
+  if _ : ¬var.validIn aig then
+    throw errInvalid
+  else if _ : ¬aig[var] matches .and _ _ then
+    throw errIsAnd
+  else
+    return aig.rewriteAnd var rhs0 rhs1
+
+-- TODO: Add convertToInput/convertToLatch/convertToAnd methods that do the right thing regardless
+-- of a variable's current type, deallocing if needed
+
+end Valaig.Aig
