Valaig/Aig.lean
@@ -1,11 +1,4 @@
 module
 
-public import Valaig.Aig.Refs
 public import Valaig.Aig.Basic
-public import Valaig.Aig.ValidIn
-public import Valaig.Aig.GetSet
-public import Valaig.Aig.WellFormed
-public import Valaig.Aig.Semantics
-public import Valaig.Aig.Iter
-public import Valaig.Aig.FromStd
-public import Valaig.Aig.Projections
+public import Valaig.Aig.Lemmas
