Valaig/Aig/Lemmas/Basic.lean
@@ -1,0 +1,561 @@
+module
+
+public import Valaig.Aig.Basic
+import all Valaig.Aig.Basic
+
+public section
+
+namespace Valaig.Aig
+variable {aig : Aig}
+
+attribute [local grind]
+  nodes inputs latches
+  size numInputs numLatches
+  maxVar nextVar newInputIdx newLatchIdx
+  numInputs numLatches numGates
+  empty
+  InputIdx.getVar InputIdx.getVar!
+  InputIdx.getLit InputIdx.getLit!
+  LatchIdx.getVar LatchIdx.getVar!
+  LatchIdx.getLit LatchIdx.getLit!
+  LatchIdx.getNext LatchIdx.getNext! LatchIdx.setNext!
+  LatchIdx.getReset LatchIdx.getReset! LatchIdx.setReset!
+  LeafIdx.validIn
+  LeafIdx.getVar LeafIdx.getVar!
+  LeafIdx.getLit LeafIdx.getLit!
+  InputIdx.convertToLatch! InputIdx.convertToAnd! InputIdx.changeIdx!
+  LatchIdx.convertToInput! LatchIdx.convertToAnd! LatchIdx.changeIdx!
+  convertAndToInput! convertAndToLatch! rewriteAnd!
+
+@[simp, grind =]
+theorem toNat_Var {var : Var} :
+    Utils.Map.AsNat.toNat var = var.idx := by
+  rfl
+
+@[simp, grind =]
+theorem ofNat_Var {nat : Nat} :
+    Utils.Map.AsNat.ofNat nat = Var.ofIdx nat := by
+  rfl
+
+@[simp, grind =]
+theorem toNat_InputIdx {idx : InputIdx} :
+    Utils.Map.AsNat.toNat idx = idx.idx := by
+  rfl
+
+@[simp, grind =]
+theorem ofNat_InputIdx {nat : Nat} :
+    Utils.Map.AsNat.ofNat nat = InputIdx.ofIdx nat := by
+  rfl
+
+@[simp, grind =]
+theorem toNat_LatchIdx {idx : LatchIdx} :
+    Utils.Map.AsNat.toNat idx = idx.idx := by
+  rfl
+
+@[simp, grind =]
+theorem ofNat_LatchIdx {nat : Nat} :
+    Utils.Map.AsNat.ofNat nat = LatchIdx.ofIdx nat := by
+  rfl
+
+@[simp, grind norm]
+theorem size_eq :
+    aig.size = aig.nodes.size := by
+  grind
+
+@[simp]
+theorem size_ne_zero :
+    aig.nodes.size > 0 :=
+  aig.sized
+
+grind_pattern size_ne_zero => aig.nodes.size
+
+@[simp, grind norm]
+theorem numInputs_eq :
+    aig.numInputs = aig.inputs.size := by
+  grind
+
+@[simp, grind norm]
+theorem numLatches_eq :
+    aig.numLatches = aig.latches.size := by
+  grind
+
+@[simp, grind =]
+theorem idx_maxVar :
+    aig.maxVar.idx = aig.size - 1 := by
+  grind
+
+@[simp, grind =]
+theorem validIn_maxVar {var : Var} :
+    var ≤ aig.maxVar ↔ var.validIn aig := by
+  grind [Var.validIn]
+
+@[simp, grind =]
+theorem idx_nextVar :
+    aig.nextVar.idx = aig.size := by
+  grind
+
+@[simp, grind .]
+theorem mem_nodes_nextVar :
+    aig.nextVar ∉ aig.nodes := by
+  grind
+
+@[simp, grind .]
+theorem mem_inputs_newInputIdx :
+    aig.newInputIdx ∉ aig.inputs := by
+  grind
+
+@[simp, grind .]
+theorem mem_latches_newLatchIdx :
+    aig.newLatchIdx ∉ aig.latches := by
+  grind
+
+@[simp, grind norm]
+theorem var_validIn {var : Var} :
+    var.validIn aig ↔ var ∈ aig.nodes := by
+  grind [Var.validIn]
+
+@[simp, grind norm]
+theorem input_validIn {idx : InputIdx} :
+    idx.validIn aig ↔ idx ∈ aig.inputs := by
+  grind [InputIdx.validIn]
+
+@[simp, grind norm]
+theorem latch_validIn {idx : LatchIdx} :
+    idx.validIn aig ↔ idx ∈ aig.latches := by
+  grind [LatchIdx.validIn]
+
+/-
+  Some basic lemmas about index validity.
+-/
+section validIn
+
+theorem validIn_mono {var var' : Var} (valid : var.validIn aig) (order : var' < var) :
+    var'.validIn aig := by
+  grind [Var.validIn]
+
+grind_pattern validIn_mono => var.validIn aig, var'.validIn aig, var' < var
+
+@[simp, grind .]
+theorem mem_nodes_constant:
+    Var.constant ∈ aig.nodes := by
+  grind [aig.sized]
+
+@[simp, grind .]
+theorem false_validIn :
+    Lit.false.validIn aig := by
+  grind
+
+@[simp, grind .]
+theorem true_validIn :
+    Lit.true.validIn aig := by
+  grind
+
+@[simp]
+theorem validIn_size {var : Var} :
+    var.idx < aig.nodes.size ↔ var.validIn aig := by
+  grind [Var.validIn]
+
+grind_pattern validIn_size => aig.nodes.size ≤ var.idx
+
+@[simp, grind =]
+theorem validIn_mapToVar {lit : Lit} {var : Var} :
+    (lit.mapToVar var).validIn aig ↔ var.validIn aig := by
+  grind
+
+@[simp, grind =]
+theorem validIn_mapTo {lit new : Lit} :
+    (lit.mapTo new).validIn aig ↔ new.validIn aig := by
+  grind
+
+end validIn
+
+@[simp, grind norm]
+theorem getElem_eq {var : Var} valid :
+    aig[var]'valid = aig.nodes[var] := by
+  cbv
+
+@[simp, grind =]
+theorem getElem_nodes_constant :
+    aig.nodes[Var.constant] = .false := by
+  grind
+
+@[simp, grind =]
+theorem getElem_false_iff_constant {var : Var} valid :
+    aig.nodes[var]'valid = .false ↔ var = .constant := by
+  grind [NodeData.toNode]
+
+@[simp, grind =]
+theorem getElem?_eq {var : Var} :
+    aig[var]? = if h : var.validIn aig then some aig[var] else none := by
+  grind [getElem?_eq_some_getElem_iff]
+
+@[simp]
+theorem mem_nodes_of_getElem?_some {var : Var} {node : Node} (h : aig[var]? = some node) :
+    var ∈ aig.nodes := by
+  grind
+
+grind_pattern mem_nodes_of_getElem?_some => aig[var]?, some node, var ∈ aig.nodes
+
+-- TODO: Write some theorems about when ! variant functions return errors, and what errors
+-- they return
+
+/-
+  `InputIdx.getVar`/`InputIdx.getVar!`.
+-/
+
+@[simp, grind norm]
+theorem input_getVar_eq {idx : InputIdx} valid :
+    idx.getVar aig valid = aig.inputs[idx].var := by
+  grind
+
+@[simp, grind =]
+theorem input_getVar!_eq {idx : InputIdx} {err : Err} valid :
+    idx.getVar! aig err = .ok (idx.getVar aig valid) := by
+  grind
+
+@[grind →]
+theorem input_getVar!_ok {idx : InputIdx} {err : Err} {var : Var} (ok : idx.getVar! aig err = .ok var) :
+    var = idx.getVar aig := by
+  grind
+
+/-
+  `InputIdx.getLit`/`InputIdx.getLit!`.
+-/
+
+@[simp, grind norm]
+theorem input_getLit_eq {idx : InputIdx} valid :
+    idx.getLit aig valid = aig.inputs[idx].var.toLit := by
+  grind
+
+@[simp, grind =]
+theorem input_getLit!_eq {idx : InputIdx} {err : Err} valid :
+    idx.getLit! aig err = .ok (idx.getLit aig valid) := by
+  grind
+
+@[grind →]
+theorem input_getLit!_ok {idx : InputIdx} {err : Err} {lit : Lit} (ok : idx.getLit! aig err = .ok lit) :
+    lit = idx.getLit aig := by
+  grind
+
+/-
+  `LatchIdx.getLit`/`LatchIdx.getLit!`.
+-/
+
+@[simp, grind norm]
+theorem latch_getVar_eq {idx : LatchIdx} valid :
+    idx.getVar aig valid = aig.latches[idx].var := by
+  grind
+
+@[simp, grind =]
+theorem latch_getVar!_eq {idx : LatchIdx} {err : Err} valid :
+    idx.getVar! aig err = .ok (idx.getVar aig valid) := by
+  grind
+
+@[grind →]
+theorem latch_getVar!_ok {idx : LatchIdx} {err : Err} {var : Var} (ok : idx.getVar! aig err = .ok var) :
+    var = idx.getVar aig := by
+  grind
+
+/-
+  `LatchIdx.getVar`/`LatchIdx.getVar!`.
+-/
+
+@[simp, grind norm]
+theorem latch_getLit_eq {idx : LatchIdx} valid :
+    idx.getLit aig valid = aig.latches[idx].var.toLit := by
+  grind
+
+@[simp, grind =]
+theorem latch_getLit!_eq {idx : LatchIdx} {err : Err} valid :
+    idx.getLit! aig err = .ok (idx.getLit aig valid) := by
+  grind
+
+@[grind →]
+theorem latch_getLit!_ok {idx : LatchIdx} {err : Err} {lit : Lit} (ok : idx.getLit! aig err = .ok lit) :
+    lit = idx.getLit aig := by
+  grind
+
+/-
+  `LatchIdx.getNext`/`LatchIdx.getNext!`.
+-/
+
+@[simp, grind norm]
+theorem getNext_eq {idx : LatchIdx} valid :
+    idx.getNext aig valid = aig.latches[idx].next := by
+  grind
+
+@[simp, grind =]
+theorem getNext!_eq {idx : LatchIdx} {err : Err} valid :
+    idx.getNext! aig err = .ok (idx.getNext aig valid) := by
+  grind
+
+@[grind →]
+theorem getNext!_ok {idx : LatchIdx} {err : Err} {lit : Lit} (ok : idx.getNext! aig err = .ok lit) :
+    lit = idx.getNext aig := by
+  grind
+
+/-
+  `LatchIdx.getReset`/`LatchIdx.getReset!`.
+-/
+
+@[simp, grind norm]
+theorem getReset_eq {idx : LatchIdx} valid :
+    idx.getReset aig valid = aig.latches[idx].reset := by
+  grind
+
+@[simp, grind =]
+theorem getReset!_eq {idx : LatchIdx} {err : Err} valid :
+    idx.getReset! aig err = .ok (idx.getReset aig valid) := by
+  grind
+
+@[grind →]
+theorem getReset!_ok {idx : LatchIdx} {err : Err} {lit : Lit} (ok : idx.getReset! aig err = .ok lit) :
+    lit = idx.getReset aig := by
+  grind
+
+/-
+  `LatchIdx.setNext!`.
+-/
+
+@[simp, grind =]
+theorem setNext!_eq {idx : LatchIdx} {next : Lit} {err : Err} valid :
+    idx.setNext! aig next err = .ok (idx.setNext aig next valid) := by
+  grind
+
+@[grind →]
+theorem setNext!_ok {idx : LatchIdx} {next : Lit} {err : Err} {aig' : Aig} (ok : idx.setNext! aig next err = .ok aig') :
+    aig' = idx.setNext aig next := by
+  grind
+
+/-
+  `LatchIdx.setReset!`
+-/
+
+@[simp, grind =]
+theorem setReset!_eq {idx : LatchIdx} {reset : Option Lit} {err : Err} valid :
+    idx.setReset! aig reset err = .ok (idx.setReset aig reset valid) := by
+  grind
+
+@[grind →]
+theorem setReset!_ok {idx : LatchIdx} {reset : Option Lit} {err : Err} {aig' : Aig} (ok : idx.setReset! aig reset err = .ok aig') :
+    aig' = idx.setReset aig reset := by
+  grind
+
+namespace LeafIdx
+
+@[simp, grind =]
+theorem asInput_eq {idx : InputIdx} :
+    (input idx).asInput = idx := by
+  rfl
+
+@[simp, grind =]
+theorem asLatch_eq {idx : LatchIdx} :
+    (latch idx).asLatch = idx := by
+  rfl
+
+@[simp, grind =]
+theorem validIn_iff {idx : LeafIdx} :
+    idx.validIn aig ↔
+    match idx with
+    | .input idx => idx.validIn aig
+    | .latch idx => idx.validIn aig := by
+  grind
+
+/-
+  `LeafIdx.getVar`/`LeafIdx.getVar!`.
+-/
+
+@[simp, grind =]
+theorem getVar_eq {idx : LeafIdx} valid :
+    idx.getVar aig valid =
+    match idx with
+    | .input idx
+    | .latch idx => idx.getVar aig := by
+  grind
+
+@[simp, grind =]
+theorem getVar!_eq {idx : LeafIdx} {err : Err} valid :
+    idx.getVar! aig err = .ok (idx.getVar aig valid) := by
+  grind
+
+@[grind →]
+theorem getVar!_ok {idx : LeafIdx} {err : Err} {var : Var} (ok : idx.getVar! aig err = .ok var) :
+    var = idx.getVar aig := by
+  grind
+
+/-
+  `LeafIdx.getLit`/`LeafIdx.getLit!`.
+-/
+
+@[simp, grind =]
+theorem getLit_eq {idx : LeafIdx} valid :
+    idx.getLit aig valid =
+    match idx with
+    | .input idx
+    | .latch idx => idx.getLit aig := by
+  grind
+
+@[simp, grind =]
+theorem getLit!_eq {idx : LeafIdx} {err : Err} valid :
+    idx.getLit! aig err = .ok (idx.getLit aig valid) := by
+  grind
+
+@[grind →]
+theorem getLit!_ok {idx : LeafIdx} {err : Err} {lit : Lit} (ok : idx.getLit! aig err = .ok lit) :
+    lit = idx.getLit aig := by
+  grind
+
+end LeafIdx
+
+/-
+  `InputIdx.convertToLatch!`.
+-/
+
+@[simp, grind =]
+theorem input_convertToLatch!_eq {idx : InputIdx} {next : Lit} {reset : Option Lit}
+    {errInvalid errVarInvalid : Err} valid varValid :
+    idx.convertToLatch! aig next reset errInvalid errVarInvalid =
+    .ok (idx.convertToLatch aig next reset valid varValid) := by
+  grind
+
+@[grind →]
+theorem input_convertToLatch!_ok {idx : InputIdx} {next : Lit} {reset : Option Lit}
+    {errInvalid errVarInvalid : Err} {res : Aig × LatchIdx}
+    (ok : idx.convertToLatch! aig next reset errInvalid errVarInvalid = .ok res) :
+    res = idx.convertToLatch aig next reset := by
+  grind
+
+/-
+  `InputIdx.convertToAnd!`.
+-/
+
+@[simp, grind =]
+theorem input_convertToAnd!_eq {idx : InputIdx} {rhs0 rhs1 : Lit}
+    {errInvalid errVarInvalid : Err} valid varValid :
+    idx.convertToAnd! aig rhs0 rhs1 errInvalid errVarInvalid =
+    .ok (idx.convertToAnd aig rhs0 rhs1 valid varValid) := by
+  grind
+
+@[grind →]
+theorem input_convertToAnd!_ok {idx : InputIdx} {rhs0 rhs1 : Lit}
+    {errInvalid errVarInvalid : Err} {aig' : Aig}
+    (ok : idx.convertToAnd! aig rhs0 rhs1 errInvalid errVarInvalid = .ok aig') :
+    aig' = idx.convertToAnd aig rhs0 rhs1 := by
+  grind
+
+/-
+  `InputIdx.changeIdx!`.
+-/
+
+@[simp, grind =]
+theorem input_changeIdx!_eq {old new : InputIdx} {errInvalid errVarInvalid errUsed : Err} valid varValid unused :
+    old.changeIdx! new aig errInvalid errVarInvalid errUsed =
+    .ok (old.changeIdx new aig valid varValid unused) := by
+  grind
+
+@[grind →]
+theorem input_changeIdx!_ok {old new : InputIdx} {errInvalid errVarInvalid errUsed : Err} {aig' : Aig}
+    (ok : old.changeIdx! new aig errInvalid errVarInvalid errUsed = .ok aig') :
+    aig' = old.changeIdx new aig := by
+  grind
+
+/-
+  `LatchIdx.convertToInput!`.
+-/
+
+@[simp, grind =]
+theorem latch_convertToInput!_eq {idx : LatchIdx} {errInvalid errVarInvalid : Err} valid varValid :
+    idx.convertToInput! aig errInvalid errVarInvalid =
+    .ok (idx.convertToInput aig valid varValid) := by
+  grind
+
+@[grind →]
+theorem latch_convertToInput!_ok {idx : LatchIdx} {errInvalid errVarInvalid : Err}
+    {res : Aig × InputIdx} (ok : idx.convertToInput! aig errInvalid errVarInvalid = .ok res) :
+    res = idx.convertToInput aig := by
+  grind
+
+/-
+  `LatchIdx.convertToAnd!`.
+-/
+
+@[simp, grind =]
+theorem latch_convertToAnd!_eq {idx : LatchIdx} {rhs0 rhs1 : Lit}
+    {errInvalid errVarInvalid : Err} valid varValid :
+    idx.convertToAnd! aig rhs0 rhs1 errInvalid errVarInvalid =
+    .ok (idx.convertToAnd aig rhs0 rhs1 valid varValid) := by
+  grind
+
+@[grind →]
+theorem latch_convertToAnd!_ok {idx : LatchIdx} {rhs0 rhs1 : Lit}
+    {errInvalid errVarInvalid : Err} {aig' : Aig}
+    (ok : idx.convertToAnd! aig rhs0 rhs1 errInvalid errVarInvalid = .ok aig') :
+    aig' = idx.convertToAnd aig rhs0 rhs1 := by
+  grind
+
+/-
+  `LatchIdx.changeIdx!`.
+-/
+
+@[simp, grind =]
+theorem latch_changeIdx!_eq {old new : LatchIdx} {errInvalid errVarInvalid errUsed : Err} valid varValid unused :
+    old.changeIdx! new aig errInvalid errVarInvalid errUsed = .ok (old.changeIdx new aig valid varValid unused) := by
+  grind
+
+@[grind →]
+theorem latch_changeIdx!_ok {old new : LatchIdx} {errInvalid errVarInvalid errUsed : Err} {aig' : Aig}
+    (ok : old.changeIdx! new aig errInvalid errVarInvalid errUsed = .ok aig') :
+    aig' = old.changeIdx new aig := by
+  grind
+
+/-
+  `convertAndToInput!`.
+-/
+
+@[simp, grind =]
+theorem convertAndToInput!_eq {var : Var} {errInvalid errIsAnd : Err} valid isAnd :
+    aig.convertAndToInput! var errInvalid errIsAnd =
+    .ok (aig.convertAndToInput var valid isAnd) := by
+  grind
+
+@[simp, grind →]
+theorem convertAndToInput!_ok {var : Var} {errInvalid errIsAnd : Err} {res : Aig × InputIdx}
+    (ok : aig.convertAndToInput! var errInvalid errIsAnd = .ok res) :
+    res = aig.convertAndToInput var := by
+  grind
+
+/-
+  `convertAndToLatch!`.
+-/
+
+@[simp, grind =]
+theorem convertAndToLatch!_eq {var : Var} {next : Lit} {reset : Option Lit}
+    {errInvalid errIsAnd : Err} valid isAnd :
+    aig.convertAndToLatch! var next reset errInvalid errIsAnd =
+    .ok (aig.convertAndToLatch var next reset valid isAnd) := by
+  grind
+
+@[simp, grind →]
+theorem convertAndToLatch!_ok {var : Var} {next : Lit} {reset : Option Lit}
+    {errInvalid errIsAnd : Err} {res : Aig × LatchIdx}
+    (ok : aig.convertAndToLatch! var next reset errInvalid errIsAnd = .ok res) :
+    res = aig.convertAndToLatch var next reset := by
+  grind
+
+/-
+  `rewriteAnd!`.
+-/
+
+@[simp, grind =]
+theorem rewriteAnd!_eq {var : Var} {rhs0 rhs1 : Lit} {errInvalid errIsAnd : Err} valid isAnd :
+    aig.rewriteAnd! var rhs0 rhs1 errInvalid errIsAnd =
+    .ok (aig.rewriteAnd var rhs0 rhs1 valid isAnd) := by
+  grind
+
+@[simp, grind →]
+theorem rewriteAnd!_ok {var : Var} {rhs0 rhs1 : Lit} {errInvalid errIsAnd : Err} {aig' : Aig}
+    (ok : aig.rewriteAnd! var rhs0 rhs1 errInvalid errIsAnd = .ok aig') :
+    aig' = aig.rewriteAnd var rhs0 rhs1 := by
+  grind
+
+end Valaig.Aig
