Valaig/Aig/Lemmas/Modify.lean
@@ -1,0 +1,660 @@
+module
+
+import all Valaig.Aig.Basic
+public import Valaig.Aig.Lemmas.Basic
+public import Valaig.Aig.Lemmas.Monotone
+
+namespace Valaig.Aig
+variable {aig : Aig}
+
+attribute [local grind] nodes inputs latches
+
+/-
+  `pushNode`.
+-/
+section pushNode
+variable {node : NodeData}
+attribute [local simp, local grind] pushNode NodeData.toNode
+
+@[simp, grind =]
+theorem nodes_pushNode :
+    (aig.pushNode node).nodes = aig.nodes.push aig.nextVar (node.toNode aig.nextVar) := by
+  apply Utils.Map.ext' <;> grind
+
+@[simp, grind =]
+theorem inputs_pushNode :
+    (aig.pushNode node).inputs = aig.inputs := by
+  grind
+
+@[simp, grind =]
+theorem latches_pushNode :
+    (aig.pushNode node).latches = aig.latches := by
+  grind
+
+@[simp, grind! .]
+theorem mono_pushNode :
+    aig ≤ aig.pushNode node := by
+  constructor <;> grind
+
+end pushNode
+
+/-
+  `setNode`.
+-/
+section setNode
+variable {var : Var} {node : NodeData} (valid : var.validIn aig)
+attribute [local simp, local grind] setNode NodeData.toNode
+
+@[simp, grind =]
+theorem nodes_setNode :
+    (aig.setNode var node valid).nodes = aig.nodes.set var (node.toNode var) := by
+  apply Utils.Map.ext' <;> grind
+
+@[simp, grind =]
+theorem inputs_setNode :
+    (aig.setNode var node valid).inputs = aig.inputs := by
+  grind
+
+@[simp, grind =]
+theorem latches_setNode :
+    (aig.setNode var node valid).latches = aig.latches := by
+  grind
+
+end setNode
+
+/-
+  `insertInput`.
+-/
+section insertInput
+variable {idx : InputIdx} {input : Input} (h : input.var ≠ .constant)
+attribute [local simp, local grind] insertInput
+
+@[simp, grind =]
+theorem nodes_insertInput :
+    (aig.insertInput idx input h).nodes = aig.nodes := by
+  grind
+
+@[simp, grind =]
+theorem inputs_insertInput :
+    (aig.insertInput idx input h).inputs = aig.inputs.insert idx input := by
+  grind
+
+@[simp, grind =]
+theorem latches_insertInput :
+    (aig.insertInput idx input h).latches = aig.latches := by
+  grind
+
+@[simp, grind! .]
+theorem mono_insertInput (unused : idx ∉ aig.inputs) :
+    aig ≤ aig.insertInput idx input h := by
+  constructor <;> grind
+
+end insertInput
+
+/-
+  `insertLatch`.
+-/
+section insertLatch
+variable {idx : LatchIdx} {latch : Latch} (h : latch.var ≠ .constant)
+attribute [local simp, local grind] insertLatch
+
+@[simp, grind =]
+theorem nodes_insertLatch :
+    (aig.insertLatch idx latch h).nodes = aig.nodes := by
+  grind
+
+@[simp, grind =]
+theorem latchs_insertLatch :
+    (aig.insertLatch idx latch h).inputs = aig.inputs := by
+  grind
+
+@[simp, grind =]
+theorem latches_insertLatch :
+    (aig.insertLatch idx latch h).latches = aig.latches.insert idx latch := by
+  grind
+
+@[simp, grind! .]
+theorem mono_insertLatch (unused : idx ∉ aig.latches) :
+    aig ≤ aig.insertLatch idx latch h := by
+  constructor <;> grind
+
+end insertLatch
+
+/-
+  `eraseInput`.
+-/
+section eraseInput
+variable {idx : InputIdx}
+attribute [local simp, local grind] eraseInput
+
+@[simp, grind =]
+theorem nodes_eraseInput :
+    (aig.eraseInput idx).nodes = aig.nodes := by
+  grind
+
+@[simp, grind =]
+theorem inputs_eraseInput :
+    (aig.eraseInput idx).inputs = aig.inputs.erase idx := by
+  grind
+
+@[simp, grind =]
+theorem latches_eraseInput :
+    (aig.eraseInput idx).latches = aig.latches := by
+  grind
+
+end eraseInput
+
+/-
+  `eraseLatch`.
+-/
+section eraseLatch
+variable {idx : LatchIdx}
+attribute [local simp, local grind] eraseLatch
+
+@[simp, grind =]
+theorem nodes_eraseLatch :
+    (aig.eraseLatch idx).nodes = aig.nodes := by
+  grind
+
+@[simp, grind =]
+theorem inputs_eraseLatch :
+    (aig.eraseLatch idx).inputs = aig.inputs := by
+  grind
+
+@[simp, grind =]
+theorem latches_eraseLatch :
+    (aig.eraseLatch idx).latches = aig.latches.erase idx := by
+  grind
+
+end eraseLatch
+
+public section
+
+/-
+  `empty`.
+-/
+section empty
+attribute [local simp, local grind] empty
+
+@[simp, grind =]
+theorem size_nodes_empty :
+    empty.nodes.size = 1 := by
+  grind
+
+@[simp, grind =]
+theorem mem_nodes_empty {var : Var} :
+    var ∈ empty.nodes ↔ var = .constant := by
+  grind
+
+@[simp, grind =]
+theorem getElem_nodes_empty {var : Var} (mem : var ∈ empty.nodes) :
+    empty.nodes[var] = .false := by
+  grind
+
+@[simp, grind =]
+theorem inputs_empty :
+    empty.inputs = .empty := by
+  grind
+
+@[simp, grind =]
+theorem latches_empty :
+    empty.latches = .empty := by
+  grind
+
+@[simp, grind .]
+theorem mono_empty (new : Aig) :
+    empty ≤ new := by
+  constructor <;> constructor <;> grind
+
+end empty
+
+/-
+  `LatchIdx.setNext`.
+-/
+section latch_setNext
+variable {idx : LatchIdx} {next : Lit} {valid : idx.validIn aig}
+attribute [local simp, local grind] LatchIdx.setNext
+
+@[simp, grind =]
+theorem nodes_setNext :
+    (idx.setNext aig next valid).nodes = aig.nodes := by
+  grind
+
+@[simp, grind =]
+theorem inputs_setNext :
+    (idx.setNext aig next valid).inputs = aig.inputs := by
+  grind
+
+@[simp, grind =]
+theorem latches_setNext :
+    (idx.setNext aig next valid).latches = aig.latches.modify idx ({ · with next }) := by
+  apply Utils.Map.ext' <;> grind
+
+end latch_setNext
+
+/-
+  `LatchIdx.setReset`.
+-/
+section latch_setReset
+variable {idx : LatchIdx} {reset : Option Lit} {valid : idx.validIn aig}
+attribute [local simp, local grind] LatchIdx.setReset
+
+@[simp, grind =]
+theorem nodes_setReset :
+    (idx.setReset aig reset valid).nodes = aig.nodes := by
+  grind
+
+@[simp, grind =]
+theorem inputs_setReset :
+    (idx.setReset aig reset valid).inputs = aig.inputs := by
+  grind
+
+@[simp, grind =]
+theorem latches_setReset :
+    (idx.setReset aig reset valid).latches = aig.latches.modify idx ({· with reset }) := by
+  apply Utils.Map.ext' <;> grind
+
+end latch_setReset
+
+/-
+ `addInput`.
+-/
+section addInput
+attribute [local simp, local grind] addInput
+
+@[simp, grind =]
+theorem snd_addInput :
+    aig.addInput.snd = aig.newInputIdx := by
+  grind
+
+@[simp, grind =]
+theorem nodes_addInput :
+    aig.addInput.fst.nodes = aig.nodes.push aig.nextVar aig.addInput.snd := by
+  grind
+
+@[simp, grind =]
+theorem inputs_addInput :
+    aig.addInput.fst.inputs = aig.inputs.push aig.newInputIdx { var := aig.nextVar } := by
+  grind
+
+@[simp, grind =]
+theorem latches_addInput :
+    aig.addInput.fst.latches = aig.latches := by
+  grind
+
+@[simp, grind! .]
+theorem mono_addInput :
+    aig ≤ aig.addInput.fst := by
+  grind
+
+end addInput
+
+/-
+ `addLatch`.
+-/
+section addLatch
+variable {next : Lit} {reset : Option Lit}
+attribute [local simp, local grind] addLatch
+
+@[simp, grind =]
+theorem snd_addLatch :
+    (aig.addLatch next reset).snd = aig.newLatchIdx := by
+  grind
+
+@[simp, grind =]
+theorem nodes_addLatch :
+    (aig.addLatch next reset).fst.nodes =
+    aig.nodes.push aig.nextVar (aig.addLatch next reset).snd := by
+  grind
+
+@[simp, grind =]
+theorem inputs_addLatch :
+    (aig.addLatch next reset).fst.inputs = aig.inputs := by
+  grind
+
+@[simp, grind =]
+theorem latches_addLatch :
+    (aig.addLatch next reset).fst.latches =
+    aig.latches.push aig.newLatchIdx { var := aig.nextVar, next, reset } := by
+  grind
+
+@[simp, grind! .]
+theorem mono_addLatch :
+    aig ≤ (aig.addLatch next reset).fst := by
+  grind
+
+end addLatch
+
+/-
+ `addAnd`.
+-/
+section addAnd
+variable {rhs0 rhs1 : Lit}
+attribute [local simp, local grind] addAnd
+
+@[simp, grind =]
+theorem snd_addAnd :
+    (aig.addAnd rhs0 rhs1).snd = aig.nextVar := by
+  grind
+
+@[simp, grind =]
+theorem nodes_addAnd (h0 : rhs0.validIn aig) (h1 : rhs1.validIn aig) :
+    (aig.addAnd rhs0 rhs1).fst.nodes =
+    aig.nodes.push aig.nextVar (.and rhs0 rhs1) := by
+  have : rhs0.var ≠ aig.nextVar ∧ rhs1.var ≠ aig.nextVar := by grind
+  grind
+
+theorem nodes_addAnd' (h0 : rhs0.var ≠ aig.nextVar) (h1 : rhs1.var ≠ aig.nextVar) :
+    (aig.addAnd rhs0 rhs1).fst.nodes =
+    aig.nodes.push aig.nextVar (.and rhs0 rhs1) := by
+  grind
+
+@[simp, grind =]
+theorem inputs_addAnd :
+    (aig.addAnd rhs0 rhs1).fst.inputs = aig.inputs := by
+  grind
+
+@[simp, grind =]
+theorem latches_addAnd :
+    (aig.addAnd rhs0 rhs1).fst.latches = aig.latches := by
+  grind
+
+@[simp, grind! .]
+theorem mono_addAnd :
+    aig ≤ (aig.addAnd rhs0 rhs1).fst := by
+  grind
+
+end addAnd
+
+/-
+ `InputIdx.convertToLatch`.
+-/
+section input_convertToLatch
+variable {idx : InputIdx} {next : Lit} {reset : Option Lit}
+variable (valid : idx.validIn aig) (varValid : (idx.getVar aig).validIn aig)
+attribute [local simp, local grind] InputIdx.convertToLatch
+
+@[simp, grind =]
+theorem snd_input_convertToLatch :
+    (idx.convertToLatch aig next reset valid varValid).snd = aig.newLatchIdx := by
+  grind
+
+@[simp, grind =]
+theorem nodes_input_convertToLatch :
+    (idx.convertToLatch aig next reset valid varValid).fst.nodes =
+    aig.nodes.set (idx.getVar aig) (idx.convertToLatch aig next reset).snd := by
+  grind
+
+@[simp, grind =]
+theorem inputs_input_convertToLatch :
+    (idx.convertToLatch aig next reset valid varValid).fst.inputs = aig.inputs.erase idx := by
+  grind
+
+@[simp, grind =]
+theorem latches_input_convertToLatch :
+    (idx.convertToLatch aig next reset valid varValid).fst.latches =
+    aig.latches.push
+      (idx.convertToLatch aig next reset).snd
+      { var := idx.getVar aig, next, reset } := by
+  grind
+
+end input_convertToLatch
+
+/-
+ `InputIdx.convertToAnd`.
+-/
+section input_convertToAnd
+variable {idx : InputIdx} {rhs0 rhs1 : Lit}
+variable (valid : idx.validIn aig) (varValid : (idx.getVar aig).validIn aig)
+attribute [local simp, local grind] InputIdx.convertToAnd
+
+
+@[simp, grind =]
+theorem nodes_input_convertToAnd (h0 : rhs0.var ≠ idx.getVar aig) (h1 : rhs1.var ≠ idx.getVar aig) :
+    (idx.convertToAnd aig rhs0 rhs1 valid varValid).nodes =
+    aig.nodes.set (idx.getVar aig) (.and rhs0 rhs1) := by
+  grind
+
+@[simp, grind =]
+theorem inputs_input_convertToAnd :
+    (idx.convertToAnd aig rhs0 rhs1 valid varValid).inputs = aig.inputs.erase idx := by
+  grind
+
+@[simp, grind =]
+theorem latches_input_convertToAnd :
+    (idx.convertToAnd aig rhs0 rhs1 valid varValid).latches = aig.latches := by
+  grind
+
+end input_convertToAnd
+
+/-
+ `InputIdx.changeIdx`.
+-/
+section input_changeIdx
+variable {old new : InputIdx}
+variable (valid : old.validIn aig) (varValid : (old.getVar aig).validIn aig) (unused : ¬new.validIn aig ∨ old = new)
+attribute [local simp, local grind] InputIdx.changeIdx
+
+@[simp, grind =]
+theorem nodes_input_changeIdx :
+    (old.changeIdx new aig valid varValid unused).nodes = aig.nodes.set (old.getVar aig) new := by
+  grind
+
+@[simp, grind =]
+theorem size_inputs_input_changeIdx :
+    (old.changeIdx new aig valid varValid unused).inputs.size = aig.inputs.size := by
+  grind
+
+@[simp, grind =]
+theorem mem_inputs_input_changeIdx {idx : InputIdx} :
+    idx ∈ (old.changeIdx new aig valid varValid unused).inputs ↔
+    (idx ∈ aig.inputs ∧ idx ≠ old) ∨ idx = new := by
+  grind
+
+@[simp, grind =]
+theorem getElem_inputs_input_changeIdx {idx : InputIdx}
+    (mem : idx ∈ (old.changeIdx new aig valid varValid unused).inputs) :
+    (old.changeIdx new aig valid varValid unused).inputs[idx] =
+    if _ : idx = new then
+      aig.inputs[old]
+    else
+      have h : idx ∈ aig.inputs := by grind
+      aig.inputs[idx]'h := by
+  grind
+
+@[simp, grind =]
+theorem latches_input_changeIdx :
+    (old.changeIdx new aig valid varValid unused).latches = aig.latches := by
+  grind
+
+end input_changeIdx
+
+/-
+ `LatchIdx.convertToInput`.
+-/
+section latch_convertToInput
+variable {idx : LatchIdx} (valid : idx.validIn aig) (varValid : (idx.getVar aig).validIn aig)
+attribute [local simp, local grind] LatchIdx.convertToInput
+
+@[simp, grind =]
+theorem snd_latch_convertToInput :
+    (idx.convertToInput aig valid varValid).snd = aig.newInputIdx := by
+  grind
+
+@[simp, grind =]
+theorem nodes_latch_convertToInput :
+    (idx.convertToInput aig valid varValid).fst.nodes =
+    aig.nodes.set (idx.getVar aig) (idx.convertToInput aig).snd := by
+  grind
+
+@[simp, grind =]
+theorem inputs_latch_convertToInput :
+    (idx.convertToInput aig valid varValid).fst.inputs =
+    aig.inputs.push (idx.convertToInput aig valid).snd { var := idx.getVar aig } := by
+  grind
+
+@[simp, grind =]
+theorem latches_latch_convertToInput :
+    (idx.convertToInput aig valid varValid).fst.latches = aig.latches.erase idx := by
+  grind
+
+end latch_convertToInput
+
+/-
+ `LatchIdx.convertToAnd`.
+-/
+section latch_convertToAnd
+variable {idx : LatchIdx} {rhs0 rhs1 : Lit}
+variable (valid : idx.validIn aig) (varValid : (idx.getVar aig).validIn aig)
+attribute [local simp, local grind] LatchIdx.convertToAnd
+
+
+@[simp, grind =]
+theorem nodes_latch_convertToAnd (h0 : rhs0.var ≠ idx.getVar aig) (h1 : rhs1.var ≠ idx.getVar aig) :
+    (idx.convertToAnd aig rhs0 rhs1 valid varValid).nodes =
+    aig.nodes.set (idx.getVar aig) (.and rhs0 rhs1) := by
+  grind
+
+@[simp, grind =]
+theorem inputs_latch_convertToAnd :
+    (idx.convertToAnd aig rhs0 rhs1 valid varValid).inputs = aig.inputs := by
+  grind
+
+@[simp, grind =]
+theorem latches_latch_convertToAnd :
+    (idx.convertToAnd aig rhs0 rhs1 valid varValid).latches = aig.latches.erase idx := by
+  grind
+
+end latch_convertToAnd
+
+/-
+ `LatchIdx.changeIdx`.
+-/
+section latch_changeIdx
+variable {old new : LatchIdx}
+variable (valid : old.validIn aig) (varValid : (old.getVar aig).validIn aig) (unused : ¬new.validIn aig ∨ old = new)
+attribute [local simp, local grind] LatchIdx.changeIdx
+
+@[simp, grind =]
+theorem nodes_latch_changeIdx :
+    (old.changeIdx new aig valid varValid unused).nodes = aig.nodes.set (old.getVar aig) new := by
+  grind
+
+@[simp, grind =]
+theorem inputs_latch_changeIdx :
+    (old.changeIdx new aig valid varValid unused).inputs = aig.inputs := by
+  grind
+
+@[simp, grind =]
+theorem size_latches_latch_changeIdx :
+    (old.changeIdx new aig valid varValid unused).latches.size = aig.latches.size := by
+  grind
+
+@[simp, grind =]
+theorem mem_latches_latch_changeIdx {idx : LatchIdx} :
+    idx ∈ (old.changeIdx new aig valid varValid unused).latches ↔
+    (idx ∈ aig.latches ∧ idx ≠ old) ∨ idx = new := by
+  grind
+
+@[simp, grind =]
+theorem getElem_latches_latch_changeIdx {idx : LatchIdx}
+    (mem : idx ∈ (old.changeIdx new aig valid varValid unused).latches) :
+    (old.changeIdx new aig valid varValid unused).latches[idx] =
+    if _ : idx = new then
+      aig.latches[old]
+    else
+      have h : idx ∈ aig.latches := by grind
+      aig.latches[idx]'h := by
+  grind
+
+end latch_changeIdx
+
+/-
+  `convertAndToInput`.
+-/
+section convertAndToInput
+variable {var : Var} (valid : var.validIn aig)
+attribute [local simp, local grind] convertAndToInput
+
+@[simp, grind =]
+theorem snd_convertAndToInput isAnd :
+    (aig.convertAndToInput var valid isAnd).snd = aig.newInputIdx := by
+  grind
+
+@[simp, grind =]
+theorem nodes_convertAndToInput isAnd :
+    (aig.convertAndToInput var valid isAnd).fst.nodes =
+    aig.nodes.set var (aig.convertAndToInput var valid isAnd).snd := by
+  grind
+
+@[simp, grind =]
+theorem inputs_convertAndToInput isAnd :
+    (aig.convertAndToInput var valid isAnd).fst.inputs =
+    aig.inputs.push aig.newInputIdx { var } := by
+  grind
+
+@[simp, grind =]
+theorem latches_convertAndToInput isAnd :
+    (aig.convertAndToInput var valid isAnd).fst.latches = aig.latches := by
+  grind
+
+end convertAndToInput
+
+/-
+  `convertAndToLatch`.
+-/
+section convertAndToLatch
+variable {var : Var} {next : Lit} {reset : Option Lit} (valid : var.validIn aig)
+attribute [local simp, local grind] convertAndToLatch
+
+@[simp, grind =]
+theorem snd_convertAndToLatch isAnd :
+    (aig.convertAndToLatch var next reset valid isAnd).snd = aig.newLatchIdx := by
+  grind
+
+@[simp, grind =]
+theorem nodes_convertAndToLatch isAnd :
+    (aig.convertAndToLatch var next reset valid isAnd).fst.nodes =
+    aig.nodes.set var (aig.convertAndToLatch var next reset valid isAnd).snd := by
+  grind
+
+@[simp, grind =]
+theorem inputs_convertAndToLatch isAnd :
+    (aig.convertAndToLatch var next reset valid isAnd).fst.inputs = aig.inputs := by
+  grind
+
+@[simp, grind =]
+theorem latches_convertAndToLatch isAnd :
+    (aig.convertAndToLatch var next reset valid isAnd).fst.latches =
+    aig.latches.push aig.newLatchIdx { var, next, reset } := by
+  grind
+
+end convertAndToLatch
+
+/-
+  `rewriteAnd`.
+-/
+section rewriteAnd
+variable {var : Var} {rhs0 rhs1 : Lit} (valid : var.validIn aig)
+attribute [local simp, local grind] rewriteAnd
+
+@[simp, grind =]
+theorem nodes_rewriteAnd isAnd (h0 : rhs0.var ≠ var) (h1 : rhs1.var ≠ var) :
+    (aig.rewriteAnd var rhs0 rhs1 valid isAnd).nodes =
+    aig.nodes.set var (.and rhs0 rhs1) := by
+  simp (disch := grind)
+
+@[simp, grind =]
+theorem inputs_rewriteAnd isAnd :
+    (aig.rewriteAnd var rhs0 rhs1 valid isAnd).inputs = aig.inputs := by
+  grind
+
+@[simp, grind =]
+theorem latches_rewriteAnd isAnd :
+    (aig.rewriteAnd var rhs0 rhs1 valid isAnd).latches = aig.latches := by
+  grind
+
+end rewriteAnd
+
+end
+end Valaig.Aig
