Valaig/Aig/Lemmas/Monotone.lean
@@ -1,0 +1,90 @@
+module
+
+public import Valaig.Aig.Lemmas.Basic
+import all Valaig.Aig.Basic
+
+public section
+namespace Valaig.Aig
+
+/--
+A pair of Aigs are monotone (represented with `old ≤ new`) if all references valid in the old Aig
+are also valid in the new Aig and all getters for these references return the same values
+-/
+structure Monotone (old new : Aig) : Prop where
+  nodes : old.nodes ≤ new.nodes
+  inputs : old.inputs ≤ new.inputs
+  latches : old.latches ≤ new.latches
+
+@[inherit_doc Monotone]
+instance : LE Aig where
+  le := Monotone
+
+@[simp]
+theorem mono_eq {old new : Aig} :
+    old.Monotone new ↔ old ≤ new := by
+  rfl
+
+instance : Std.IsPreorder Aig := by
+  apply Std.IsPreorder.of_le
+  <;> constructor
+  <;> grind [=_ mono_eq, Monotone]
+
+attribute [grind norm] mono_eq
+
+section Monotone
+variable {old new : Aig} (mono : old ≤ new)
+include mono
+
+@[simp, grind .]
+theorem mono_nodes_mono :
+    old.nodes ≤ new.nodes :=
+  mono.nodes
+
+@[simp, grind .]
+theorem mono_inputs_mono :
+    old.inputs ≤ new.inputs :=
+  mono.inputs
+
+@[simp, grind .]
+theorem mono_latches_mono :
+    old.latches ≤ new.latches :=
+  mono.latches
+
+@[simp, grind .]
+theorem mem_nodes_mono {var : Var} (mem : var ∈ old.nodes) :
+    var ∈ new.nodes := by
+  grind [mono.nodes]
+
+@[simp, grind .]
+theorem mem_inputs_mono {idx : InputIdx} (mem : idx ∈ old.inputs) :
+    idx ∈ new.inputs := by
+  grind [mono.inputs]
+
+@[simp, grind .]
+theorem mem_latches_mono {idx : LatchIdx} (mem : idx ∈ old.latches) :
+    idx ∈ new.latches := by
+  grind [mono.latches]
+
+@[simp]
+theorem getElem_nodes_mono {var : Var} (mem : var ∈ old.nodes) :
+    new.nodes[var] = old.nodes[var] := by
+  grind [mono.nodes]
+
+grind_pattern getElem_nodes_mono => new.nodes[var], old ≤ new
+
+@[simp]
+theorem getElem_inputs_mono {idx : InputIdx} (mem : idx ∈ old.inputs) :
+    new.inputs[idx] = old.inputs[idx] := by
+  grind [mono.inputs]
+
+grind_pattern getElem_inputs_mono => new.inputs[idx], old ≤ new
+
+@[simp]
+theorem getElem_latches_mono {idx : LatchIdx} (mem : idx ∈ old.latches) :
+    new.latches[idx] = old.latches[idx] := by
+  grind [mono.latches]
+
+grind_pattern getElem_latches_mono => new.latches[idx], old ≤ new
+
+end Monotone
+end Valaig.Aig
