Valaig/Aig/Lemmas/WellFormed.lean
@@ -1,0 +1,1476 @@
+module
+
+public import Valaig.Aig.Lemmas.Basic
+public import Valaig.Aig.Lemmas.Modify
+public import Valaig.Aig.Lemmas.Monotone
+import all Valaig.Aig.Basic
+import all Valaig.Aig.Lemmas.Modify
+
+public section
+namespace Valaig.Aig
+variable {aig : Aig}
+
+/-
+To try to prevent too much pollution of grind patterns, we try to set up the following strategy:
+- WellFormed and individual wellformedness predicates (e.g. InputsValid) should automatically
+  propagate forwards and backwards over terms preserving them, however WellFormed should not
+  automatically cast to individual predicates.
+- Specific uses of each predicate are defined as theorems that require that predicate as argument
+  and match on specific outputs.
+- Theorems to bridge from WellFormed to each predicate exist but are only triggered if both
+  parts appear (as should have been triggered by the above rules).
+-/
+
+/--
+  All input indices point to an input in the Aig.
+-/
+@[expose, local grind, local simp]
+def InputsValid (aig : Aig) : Prop :=
+  ∀ idx (_ : idx ∈ aig.inputs),
+  ∃ (_ : aig.inputs[idx].var ∈ aig.nodes),
+    aig.nodes[aig.inputs[idx].var] = idx
+
+@[simp, grind .]
+theorem WF.var_inputs_mem_nodes {inputsValid : aig.InputsValid} {idx : InputIdx} (mem : idx ∈ aig.inputs) :
+    (aig.inputs[idx]'mem).var ∈ aig.nodes := by
+  grind
+
+@[simp, grind =]
+theorem WF.nodes_var_inputs_eq {inputsValid : aig.InputsValid} {idx : InputIdx} (mem : idx ∈ aig.inputs) :
+    aig.nodes[(aig.inputs[idx]'mem).var] = idx := by
+  grind
+
+/--
+  All inputs in the Aig point to a corresponding input index.
+-/
+@[expose, local grind, local simp]
+def InputIdxsValid (aig : Aig) : Prop :=
+  ∀ var (_ : var ∈ aig.nodes) idx,
+    aig[var] = .input idx → ∃ _, aig.inputs[idx].var = var
+
+@[simp]
+theorem WF.mem_inputs_of_node {inputIdxsValid : aig.InputIdxsValid} {var : Var} {idx : InputIdx}
+    (mem : var ∈ aig.nodes) (eq : aig[var] = .input idx) :
+    idx ∈ aig.inputs := by
+  grind
+
+grind_pattern WF.mem_inputs_of_node => idx ∈ aig.inputs, aig[var], Node.input idx
+
+@[simp]
+theorem WF.var_inputs_of_node {inputIdxsValid : aig.InputIdxsValid} {var : Var} {idx : InputIdx}
+    (mem : var ∈ aig.nodes) (eq : aig[var] = .input idx) :
+    aig.inputs[idx].var = var := by
+  grind
+
+grind_pattern WF.var_inputs_of_node => idx ∈ aig.inputs, aig[var], Node.input idx
+
+/--
+  All latch indices point to a latch in the Aig.
+-/
+@[expose, local grind, local simp]
+def LatchesValid (aig : Aig) : Prop :=
+  ∀ idx (_ : idx ∈ aig.latches),
+  ∃ (_ : aig.latches[idx].var ∈ aig.nodes),
+    aig.nodes[aig.latches[idx].var] = idx
+
+@[simp, grind .]
+theorem WF.var_latches_mem_nodes {latchesValid : aig.LatchesValid} {idx : LatchIdx} (mem : idx ∈ aig.latches) :
+    (aig.latches[idx]'mem).var ∈ aig.nodes := by
+  grind
+
+@[simp, grind =]
+theorem WF.nodes_var_latches_eq {latchesValid : aig.LatchesValid} {idx : LatchIdx} (mem : idx ∈ aig.latches) :
+    aig.nodes[(aig.latches[idx]'mem).var] = idx := by
+  grind
+
+/--
+  All latches in the Aig point to a corresponding latch index.
+-/
+@[expose, local grind, local simp]
+def LatchIdxsValid (aig : Aig) : Prop :=
+  ∀ var (_ : var ∈ aig.nodes) idx,
+    aig[var] = .latch idx → ∃ _, aig.latches[idx].var = var
+
+@[simp]
+theorem WF.mem_latches_of_node {latchIdxsValid : aig.LatchIdxsValid} {var : Var} {idx : LatchIdx}
+    (mem : var ∈ aig.nodes) (eq : aig[var] = .latch idx) :
+    idx ∈ aig.latches := by
+  grind
+
+grind_pattern WF.mem_latches_of_node => idx ∈ aig.latches, aig[var], Node.latch idx
+
+@[simp]
+theorem WF.var_latches_of_node {latchIdxsValid : aig.LatchIdxsValid} {var : Var} {idx : LatchIdx}
+    (mem : var ∈ aig.nodes) (eq : aig[var] = .latch idx) :
+    aig.latches[idx].var = var := by
+  grind
+
+grind_pattern WF.var_latches_of_node => idx ∈ aig.latches, aig[var], Node.latch idx
+
+/-
+  Equivalent of `getElem_nodes_LatchesValid` on leaves.
+-/
+@[simp]
+theorem WF.getVar_LeafIdxsValid {inputsValid : aig.InputsValid} {latchesValid : aig.LatchesValid}
+    {idx : LeafIdx} (valid : idx.validIn aig) :
+    idx.getVar aig valid ∈ aig.nodes := by
+  grind
+
+grind_pattern WF.getVar_LeafIdxsValid => idx.getVar aig valid ∈ aig.nodes
+
+/--
+  All latch reset literals are valid in the Aig.
+  This follows from `LatchesValid` and `AcyclicResets`.
+-/
+@[expose, local grind, local simp]
+def ResetsValid (aig : Aig) : Prop :=
+  ∀ idx (_ : idx ∈ aig.latches),
+    match aig.latches[idx].reset with
+    | none => True
+    | some lit => lit.validIn aig
+
+@[simp]
+theorem WF.mem_nodes_reset {resetsValid : aig.ResetsValid} {idx : LatchIdx} (mem : idx ∈ aig.latches)
+    {lit : Lit} (isSome : aig.latches[idx].reset = some lit) :
+    lit.validIn aig := by
+  grind
+
+grind_pattern WF.mem_nodes_reset => aig.latches[idx].reset, some lit, lit.validIn aig
+
+/--
+  All latch next state literals are valid in the Aig.
+-/
+@[expose, local grind, local simp]
+def NextsValid (aig : Aig) : Prop :=
+  ∀ idx (_ : idx ∈ aig.latches),
+    aig.latches[idx].next.validIn aig
+
+@[simp, grind .]
+theorem WF.mem_nodes_next {nextsValid : aig.NextsValid} {idx : LatchIdx} (mem : idx ∈ aig.latches) :
+    aig.latches[idx].next.validIn aig := by
+  grind
+
+/--
+  The gates of the Aig are acyclic.
+  This is enforced by requiring each gate's inputs to have lower variable
+  indices than themselves.
+-/
+@[expose, local grind, local simp]
+def AcyclicGates (aig : Aig) : Prop :=
+  ∀ {var : Var} {rhs0 rhs1} (mem : var ∈ aig.nodes),
+    aig.nodes[var] = .and rhs0 rhs1 → rhs0.var < var ∧ rhs1.var < var
+
+section AcyclicGates
+variable {acyclicGates : aig.AcyclicGates} {var var' : Var} {rhs0 rhs1 : Lit}
+variable (valid : var.validIn aig) (eq : aig.nodes[var] = .and rhs0 rhs1)
+include acyclicGates valid eq
+
+@[simp]
+theorem WF.rhs0_lt_and :
+    rhs0.var < var := by
+  grind
+
+@[simp]
+theorem WF.rhs1_lt_and :
+    rhs1.var < var := by
+  grind
+
+theorem WF.rhs0_lt_and_of_le (lt : var ≤ var') :
+    rhs0.var < var' := by
+  grind
+
+grind_pattern WF.rhs0_lt_and_of_le => rhs0.var < var', Node.and rhs0 rhs1, aig.nodes[var]
+grind_pattern WF.rhs0_lt_and_of_le => rhs0.var ≤ var', Node.and rhs0 rhs1, aig.nodes[var]
+
+theorem WF.rhs1_lt_and_of_le (lt : var ≤ var') :
+    rhs1.var < var' := by
+  grind
+
+grind_pattern WF.rhs1_lt_and_of_le => rhs1.var < var', Node.and rhs0 rhs1, aig.nodes[var]
+grind_pattern WF.rhs1_lt_and_of_le => rhs1.var ≤ var', Node.and rhs0 rhs1, aig.nodes[var]
+
+@[simp]
+theorem WF.rhs0_mem_nodes_and :
+    rhs0.var ∈ aig.nodes := by
+  grind
+
+grind_pattern WF.rhs0_mem_nodes_and => rhs0.var.validIn aig, Node.and rhs0 rhs1, aig.nodes[var]
+
+@[simp]
+theorem WF.rhs1_mem_nodes_and :
+    rhs1.var ∈ aig.nodes := by
+  grind
+
+grind_pattern WF.rhs1_mem_nodes_and => rhs1.var.validIn aig, Node.and rhs0 rhs1, aig.nodes[var]
+
+end AcyclicGates
+
+/--
+  The reset function of the Aig is acyclic.
+  This is enfoced by requiring each latch's reset to have a lower variable
+  index than the latch's output.
+-/
+@[expose, local grind, local simp]
+def AcyclicResets (aig : Aig) : Prop :=
+  ∀ idx (_ : idx ∈ aig.latches),
+    match aig.latches[idx].reset with
+    | none => True
+    | some lit => lit.var < aig.latches[idx].var
+
+theorem WF.ResetsValid_of_LatchesValid_AcyclicReset {aig : Aig}
+    (latchesValid : aig.LatchesValid)
+    (acyclicResets : aig.AcyclicResets) :
+    aig.ResetsValid := by
+  grind
+
+@[simp]
+theorem WF.reset_lt_var (acyclicResets : aig.AcyclicResets) {idx : LatchIdx} (mem : idx ∈ aig.latches)
+    {lit : Lit} (isSome : aig.latches[idx].reset = some lit) :
+    lit.var < aig.latches[idx].var := by
+  grind
+
+theorem WF.reset_lt_var_of_le (acyclicResets : aig.AcyclicResets) {var : Var} {idx : LatchIdx}
+    (mem : idx ∈ aig.latches) (lt : aig.latches[idx].var ≤ var)
+    {lit : Lit} (isSome : aig.latches[idx].reset = some lit) :
+    lit.var < var := by
+  grind
+
+grind_pattern WF.reset_lt_var_of_le => aig.latches[idx], some lit, lit.var < var
+grind_pattern WF.reset_lt_var_of_le => aig.latches[idx], some lit, lit.var ≤ var
+
+/--
+  All indices within the Aig are valid and the gates and reset function are
+  acyclic, allowing the definition of semantics.
+-/
+@[local grind]
+structure WF (aig : Aig) : Prop where
+  inputsValid : aig.InputsValid
+  inputIdxsValid : aig.InputIdxsValid
+
+  latchesValid : aig.LatchesValid
+  latchIdxsValid : aig.LatchIdxsValid
+  resetsValid : aig.ResetsValid
+  nextsValid : aig.NextsValid
+
+  acyclicGates : aig.AcyclicGates
+  acyclicResets : aig.AcyclicResets
+
+namespace WF
+
+section triggers
+variable (wf : aig.WF)
+include wf
+
+theorem InputsValid_of_WF    : aig.InputsValid    := wf.inputsValid
+theorem InputIdxsValid_of_WF : aig.InputIdxsValid := wf.inputIdxsValid
+theorem LatchesValid_of_WF   : aig.LatchesValid   := wf.latchesValid
+theorem LatchIdxsValid_of_WF : aig.LatchIdxsValid := wf.latchIdxsValid
+theorem ResetsValid_of_WF    : aig.ResetsValid    := wf.resetsValid
+theorem NextsValid_of_WF     : aig.NextsValid     := wf.nextsValid
+theorem AcyclicGates_of_WF   : aig.AcyclicGates   := wf.acyclicGates
+theorem AcyclicResets_of_WF  : aig.AcyclicResets  := wf.acyclicResets
+
+grind_pattern AcyclicResets_of_WF  => aig.WF, aig.AcyclicResets
+grind_pattern AcyclicGates_of_WF   => aig.WF, aig.AcyclicGates
+grind_pattern InputsValid_of_WF    => aig.WF, aig.InputsValid
+grind_pattern InputIdxsValid_of_WF => aig.WF, aig.InputIdxsValid
+grind_pattern LatchesValid_of_WF   => aig.WF, aig.LatchesValid
+grind_pattern LatchIdxsValid_of_WF => aig.WF, aig.LatchIdxsValid
+grind_pattern ResetsValid_of_WF    => aig.WF, aig.ResetsValid
+grind_pattern NextsValid_of_WF     => aig.WF, aig.NextsValid
+
+end triggers
+
+/-
+  `empty`.
+-/
+section empty
+
+@[simp, grind .] theorem InputsValid_empty    : empty.InputsValid    := by grind
+@[simp, grind .] theorem InputIdxsValid_empty : empty.InputIdxsValid := by grind
+@[simp, grind .] theorem LatchesValid_empty   : empty.LatchesValid   := by grind
+@[simp, grind .] theorem LatchIdxsValid_empty : empty.LatchIdxsValid := by grind
+@[simp, grind .] theorem ResetsValid_empty    : empty.ResetsValid    := by grind
+@[simp, grind .] theorem NextsValid_empty     : empty.NextsValid     := by grind
+@[simp, grind .] theorem AcyclicGates_empty   : empty.AcyclicGates   := by grind
+@[simp, grind .] theorem AcyclicResets_empty  : empty.AcyclicResets  := by grind
+@[simp, grind .] theorem WF_empty             : empty.WF             := by grind
+
+end empty
+
+/-
+  `LatchIdx.setNext`.
+-/
+section latch_setNext
+variable {idx : LatchIdx} {next : Lit} (valid : idx.validIn aig)
+
+@[simp, grind .]
+theorem InputsValid_setNext
+    (inputsValid : aig.InputsValid) :
+    (idx.setNext aig next).InputsValid := by
+  grind
+
+@[simp, grind .]
+theorem InputIdxsValid_setNext
+    (inputIdxsValid : aig.InputIdxsValid) :
+    (idx.setNext aig next valid).InputIdxsValid := by
+  grind
+
+@[simp, grind .]
+theorem LatchesValid_setNext
+    (latchesValid : aig.LatchesValid) :
+    (idx.setNext aig next valid).LatchesValid := by
+  grind
+
+@[simp, grind .]
+theorem LatchIdxsValid_setNext
+    (latchIdxsValid : aig.LatchIdxsValid) :
+    (idx.setNext aig next valid).LatchIdxsValid := by
+  grind
+
+@[simp, grind .]
+theorem ResetsValid_setNext
+    (resetsValid : aig.ResetsValid) :
+    (idx.setNext aig next valid).ResetsValid := by
+  grind
+
+@[simp, grind .]
+theorem NextsValid_setNext
+    (nextsValid : aig.NextsValid)
+    (nextValid : next.validIn aig) :
+    (idx.setNext aig next valid).NextsValid := by
+  grind
+
+@[simp, grind .]
+theorem AcyclicGates_setNext
+    (acyclicGates : aig.AcyclicGates) :
+    (idx.setNext aig next valid).AcyclicGates := by
+  grind
+
+@[simp, grind .]
+theorem AcyclicResets_setNext
+    (acyclicResets : aig.AcyclicResets) :
+    (idx.setNext aig next valid).AcyclicResets := by
+  grind
+
+@[simp, grind .]
+theorem setNext
+    (wellFormed : aig.WF)
+    (nextValid : next.validIn aig) :
+    (idx.setNext aig next valid).WF := by
+  grind
+
+end latch_setNext
+
+/-
+  `LatchIdx.setReset`.
+-/
+section latch_setReset
+variable {idx : LatchIdx} {reset : Option Lit} (valid : idx.validIn aig)
+
+@[simp, grind .]
+theorem InputsValid_setReset
+    (inputsValid : aig.InputsValid) :
+    (idx.setReset aig reset).InputsValid := by
+  grind
+
+@[simp, grind .]
+theorem InputIdxsValid_setReset
+    (inputIdxsValid : aig.InputIdxsValid) :
+    (idx.setReset aig reset valid).InputIdxsValid := by
+  grind
+
+@[simp, grind .]
+theorem LatchesValid_setReset
+    (latchesValid : aig.LatchesValid) :
+    (idx.setReset aig reset valid).LatchesValid := by
+  grind
+
+@[simp, grind .]
+theorem LatchIdxsValid_setReset
+    (latchIdxsValid : aig.LatchIdxsValid) :
+    (idx.setReset aig reset valid).LatchIdxsValid := by
+  grind
+
+@[simp]
+theorem ResetsValid_setReset_none
+    (resetsValid : aig.ResetsValid) :
+    (idx.setReset aig none valid).ResetsValid := by
+  grind
+
+@[simp]
+theorem ResetsValid_setReset_some {reset : Lit}
+    (resetsValid : aig.ResetsValid)
+    (resetValid : reset.validIn aig) :
+    (idx.setReset aig reset valid).ResetsValid := by
+  grind
+
+@[grind .]
+theorem ResetsValid_setReset
+    (resetsValid : aig.ResetsValid)
+    (resetValid :
+      match reset with
+      | none => True
+      | some lit => lit.validIn aig) :
+    (idx.setReset aig reset valid).ResetsValid := by
+  grind
+
+@[simp, grind .]
+theorem NextsValid_setReset
+    (nextsValid : aig.NextsValid) :
+    (idx.setReset aig reset valid).NextsValid := by
+  grind
+
+@[simp, grind .]
+theorem AcyclicGates_setReset
+    (acyclicGates : aig.AcyclicGates) :
+    (idx.setReset aig reset valid).AcyclicGates := by
+  grind
+
+@[simp]
+theorem AcyclicResets_setReset_none
+    (acyclicResets : aig.AcyclicResets) :
+    (idx.setReset aig none valid).AcyclicResets := by
+  grind
+
+@[simp]
+theorem AcyclicResets_setReset_some {reset : Lit}
+    (acyclicResets : aig.AcyclicResets)
+    (resetAcyclic : reset.var < idx.getVar aig) :
+    (idx.setReset aig reset valid).AcyclicResets := by
+  grind
+
+@[grind .]
+theorem AcyclicResets_setReset
+    (acyclicResets : aig.AcyclicResets)
+    (resetAcyclic :
+      match reset with
+      | none => True
+      | some lit => lit.var < idx.getVar aig) :
+    (idx.setReset aig reset valid).AcyclicResets := by
+  grind
+
+@[simp]
+theorem setReset_none
+    (wellFormed : aig.WF) :
+    (idx.setReset aig none valid).WF := by
+  grind
+
+@[simp]
+theorem setReset_some {reset : Lit}
+    (wellFormed : aig.WF)
+    (resetAcyclic : reset.var < idx.getVar aig) :
+    (idx.setReset aig reset valid).WF := by
+  grind
+
+@[grind .]
+theorem setReset
+    (wellFormed : aig.WF)
+    (resetAcyclic :
+      match reset with
+      | none => True
+      | some lit => lit.var < idx.getVar aig) :
+    (idx.setReset aig reset valid).WF := by
+  grind
+
+end latch_setReset
+
+/-
+  `addInput`
+-/
+section addInput
+
+@[simp, grind .]
+theorem InputsValid_addInput
+    (inputsValid : aig.InputsValid) :
+    aig.addInput.fst.InputsValid := by
+  grind
+
+@[simp, grind .]
+theorem InputIdxsValid_addInput
+    (inputIdxsValid : aig.InputIdxsValid) :
+    aig.addInput.fst.InputIdxsValid := by
+  grind
+
+@[simp, grind .]
+theorem LatchesValid_addInput
+    (latchesValid : aig.LatchesValid) :
+    aig.addInput.fst.LatchesValid := by
+  grind
+
+@[simp, grind .]
+theorem LatchIdxsValid_addInput
+    (latchIdxsValid : aig.LatchIdxsValid) :
+    aig.addInput.fst.LatchIdxsValid := by
+  grind
+
+@[simp, grind .]
+theorem ResetsValid_addInput
+    (resetsValid : aig.ResetsValid) :
+    aig.addInput.fst.ResetsValid := by
+  grind
+
+@[simp, grind .]
+theorem NextsValid_addInput
+    (nextsValid : aig.NextsValid) :
+    aig.addInput.fst.NextsValid := by
+  grind
+
+@[simp, grind .]
+theorem AcyclicGates_addInput
+    (acyclicGates : aig.AcyclicGates) :
+    aig.addInput.fst.AcyclicGates := by
+  grind
+
+@[simp, grind .]
+theorem AcyclicResets_addInput
+    (acyclicResets : aig.AcyclicResets) :
+    aig.addInput.fst.AcyclicResets := by
+  grind
+
+@[simp, grind .]
+theorem addInput
+    (wellFormed : aig.WF) :
+    aig.addInput.fst.WF := by
+  grind
+
+end addInput
+
+/-
+  `addLatch`
+-/
+section addLatch
+variable {next : Lit} {reset : Option Lit}
+
+@[simp, grind .]
+theorem InputsValid_addLatch
+    (inputsValid : aig.InputsValid) :
+    (aig.addLatch next reset).fst.InputsValid := by
+  grind
+
+@[simp, grind .]
+theorem InputIdxsValid_addLatch
+    (inputIdxsValid : aig.InputIdxsValid) :
+    (aig.addLatch next reset).fst.InputIdxsValid := by
+  grind
+
+@[simp, grind .]
+theorem LatchesValid_addLatch
+    (latchesValid : aig.LatchesValid) :
+    (aig.addLatch next reset).fst.LatchesValid := by
+  grind
+
+@[simp, grind .]
+theorem LatchIdxsValid_addLatch
+    (latchIdxsValid : aig.LatchIdxsValid) :
+    (aig.addLatch next reset).fst.LatchIdxsValid := by
+  grind
+
+@[simp]
+theorem ResetsValid_addLatch_none
+    (resetsValid : aig.ResetsValid) :
+    (aig.addLatch next none).fst.ResetsValid := by
+  grind
+
+@[simp]
+theorem ResetsValid_addLatch_some {reset : Lit}
+    (resetsValid : aig.ResetsValid)
+    (resetValid : reset.validIn aig) :
+    (aig.addLatch next reset).fst.ResetsValid := by
+  grind
+
+@[grind .]
+theorem ResetsValid_addLatch
+    (resetsValid : aig.ResetsValid)
+    (resetValid :
+      match reset with
+      | none => True
+      | some lit => lit.validIn aig) :
+    (aig.addLatch next reset).fst.ResetsValid := by
+  grind
+
+@[simp, grind .]
+theorem NextsValid_addLatch
+    (nextsValid : aig.NextsValid)
+    (nextValid : next.validIn aig) :
+    (aig.addLatch next reset).fst.NextsValid := by
+  grind
+
+@[simp, grind .]
+theorem AcyclicGates_addLatch
+    (acyclicGates : aig.AcyclicGates) :
+    (aig.addLatch next reset).fst.AcyclicGates := by
+  grind
+
+@[simp]
+theorem AcyclicResets_addLatch_none
+    (acyclicResets : aig.AcyclicResets) :
+    (aig.addLatch next none).fst.AcyclicResets := by
+  grind
+
+@[simp]
+theorem AcyclicResets_addLatch_some {reset : Lit}
+    (acyclicResets : aig.AcyclicResets)
+    (resetValid : reset.validIn aig) :
+    (aig.addLatch next reset).fst.AcyclicResets := by
+  grind
+
+@[grind .]
+theorem AcyclicResets_addLatch
+    (acyclicResets : aig.AcyclicResets)
+    (resetValid :
+      match reset with
+      | none => True
+      | some lit => lit.validIn aig) :
+    (aig.addLatch next reset).fst.AcyclicResets := by
+  grind
+
+@[simp]
+theorem addLatch_none
+    (wellFormed : aig.WF)
+    (nextValid : next.validIn aig) :
+    (aig.addLatch next none).fst.WF := by
+  grind
+
+@[simp]
+theorem addLatch_some {reset : Lit}
+    (wellFormed : aig.WF)
+    (nextValid : next.validIn aig)
+    (resetValid : reset.validIn aig) :
+    (aig.addLatch next reset).fst.WF := by
+  grind
+
+@[grind .]
+theorem addLatch
+    (wellFormed : aig.WF)
+    (nextValid : next.validIn aig)
+    (resetValid :
+      match reset with
+      | none => True
+      | some lit => lit.validIn aig) :
+    (aig.addLatch next reset).fst.WF := by
+  grind
+
+end addLatch
+
+/-
+  `addAnd`
+-/
+section addAnd
+variable {rhs0 rhs1 : Lit}
+
+@[simp, grind .]
+theorem InputsValid_addAnd
+    (inputsValid : aig.InputsValid) :
+    (aig.addAnd rhs0 rhs1).fst.InputsValid := by
+  grind
+
+@[simp, grind .]
+theorem InputIdxsValid_addAnd
+    (inputIdxsValid : aig.InputIdxsValid)
+    (h0 : rhs0.validIn aig)
+    (h1 : rhs1.validIn aig) :
+    (aig.addAnd rhs0 rhs1).fst.InputIdxsValid := by
+  grind
+
+theorem InputIdxsValid_addAnd'
+    (inputIdxsValid : aig.InputIdxsValid)
+    (h0 : rhs0.var ≠ aig.nextVar)
+    (h1 : rhs1.var ≠ aig.nextVar) :
+    (aig.addAnd rhs0 rhs1).fst.InputIdxsValid := by
+    grind [nodes_addAnd']
+
+@[simp, grind .]
+theorem LatchesValid_addAnd
+    (latchesValid : aig.LatchesValid) :
+    (aig.addAnd rhs0 rhs1).fst.LatchesValid := by
+  grind
+
+@[simp, grind .]
+theorem LatchIdxsValid_addAnd
+    (latchIdxsValid : aig.LatchIdxsValid)
+    (h0 : rhs0.validIn aig)
+    (h1 : rhs1.validIn aig) :
+    (aig.addAnd rhs0 rhs1).fst.LatchIdxsValid := by
+  grind
+
+theorem LatchIdxsValid_addAnd'
+    (inputIdxsValid : aig.LatchIdxsValid)
+    (h0 : rhs0.var ≠ aig.nextVar)
+    (h1 : rhs1.var ≠ aig.nextVar) :
+    (aig.addAnd rhs0 rhs1).fst.LatchIdxsValid := by
+    grind [nodes_addAnd']
+
+@[simp, grind .]
+theorem ResetsValid_addAnd
+    (resetsValid : aig.ResetsValid) :
+    (aig.addAnd rhs0 rhs1).fst.ResetsValid := by
+  grind
+
+@[simp, grind .]
+theorem NextsValid_addAnd
+    (nextsValid : aig.NextsValid) :
+    (aig.addAnd rhs0 rhs1).fst.NextsValid := by
+  grind
+
+@[simp, grind .]
+theorem AcyclicGates_addAnd
+    (acyclicGates : aig.AcyclicGates)
+    (h0 : rhs0.validIn aig)
+    (h1 : rhs1.validIn aig) :
+    (aig.addAnd rhs0 rhs1).fst.AcyclicGates := by
+  grind
+
+@[simp, grind .]
+theorem AcyclicResets_addAnd
+    (acyclicResets : aig.AcyclicResets) :
+    (aig.addAnd rhs0 rhs1).fst.AcyclicResets := by
+  grind
+
+@[simp, grind .]
+theorem addAnd
+    (wellFormed : aig.WF)
+    (h0 : rhs0.validIn aig)
+    (h1 : rhs1.validIn aig) :
+    (aig.addAnd rhs0 rhs1).fst.WF := by
+  grind
+
+end addAnd
+
+/-
+  `InputIdx.convertToLatch`
+-/
+section input_convertToLatch
+variable {idx : InputIdx} {next : Lit} {reset : Option Lit}
+variable (valid : idx.validIn aig) (varValid : (idx.getVar aig valid).validIn aig)
+
+@[simp, grind .]
+theorem InputsValid_input_convertToLatch
+    (inputsValid : aig.InputsValid) :
+    (idx.convertToLatch aig next reset valid varValid).fst.InputsValid := by
+  grind
+
+@[simp, grind .]
+theorem InputIdxsValid_input_convertToLatch
+    (inputIdxsValid : aig.InputIdxsValid) :
+    (idx.convertToLatch aig next reset valid varValid).fst.InputIdxsValid := by
+  grind
+
+@[simp, grind .]
+theorem LatchesValid_input_convertToLatch
+    (latchesValid : aig.LatchesValid)
+    (inputsValid  : aig.InputsValid) :
+    (idx.convertToLatch aig next reset valid varValid).fst.LatchesValid := by
+  grind
+
+@[simp, grind .]
+theorem LatchIdxsValid_input_convertToLatch
+    (latchIdxsValid : aig.LatchIdxsValid) :
+    (idx.convertToLatch aig next reset valid varValid).fst.LatchIdxsValid := by
+  grind
+
+@[simp]
+theorem ResetsValid_input_convertToLatch_none
+    (resetsValid : aig.ResetsValid) :
+    (idx.convertToLatch aig next none valid varValid).fst.ResetsValid := by
+  grind
+
+@[simp]
+theorem ResetsValid_input_convertToLatch_some {reset : Lit}
+    (resetsValid : aig.ResetsValid)
+    (resetValid : reset.validIn aig) :
+    (idx.convertToLatch aig next reset valid varValid).fst.ResetsValid := by
+  grind
+
+@[grind .]
+theorem ResetsValid_input_convertToLatch
+    (resetsValid : aig.ResetsValid)
+    (resetValid :
+      match reset with
+      | none => True
+      | some lit => lit.validIn aig) :
+    (idx.convertToLatch aig next reset valid varValid).fst.ResetsValid := by
+  grind
+
+@[simp, grind .]
+theorem NextsValid_input_convertToLatch
+    (nextsValid : aig.NextsValid)
+    (nextValid : next.validIn aig) :
+    (idx.convertToLatch aig next reset valid varValid).fst.NextsValid := by
+  grind
+
+@[simp, grind .]
+theorem AcyclicGates_input_convertToLatch
+    (acyclicGates : aig.AcyclicGates) :
+    (idx.convertToLatch aig next reset valid varValid).fst.AcyclicGates := by
+  grind
+
+@[simp]
+theorem AcyclicResets_input_convertToLatch_none
+    (acyclicResets : aig.AcyclicResets) :
+    (idx.convertToLatch aig next none valid varValid).fst.AcyclicResets := by
+  grind
+
+@[simp]
+theorem AcyclicResets_input_convertToLatch_some {reset : Lit}
+    (acyclicResets : aig.AcyclicResets)
+    (resetAcyclic : reset.var < idx.getVar aig) :
+    (idx.convertToLatch aig next reset valid varValid).fst.AcyclicResets := by
+  grind
+
+@[grind .]
+theorem AcyclicResets_input_convertToLatch
+    (acyclicResets : aig.AcyclicResets)
+    (resetAcyclic :
+      match reset with
+      | none => True
+      | some lit => lit.var < idx.getVar aig) :
+    (idx.convertToLatch aig next reset valid varValid).fst.AcyclicResets := by
+  grind
+
+@[simp]
+theorem input_convertToLatch_none
+    (wellFormed : aig.WF)
+    (nextValid : next.validIn aig) :
+    (idx.convertToLatch aig next none valid varValid).fst.WF := by
+  grind
+
+@[simp]
+theorem input_convertToLatch_some {reset : Lit}
+    (wellFormed : aig.WF)
+    (nextValid : next.validIn aig)
+    (resetAcyclic : reset.var < idx.getVar aig) :
+    (idx.convertToLatch aig next reset valid varValid).fst.WF := by
+  grind
+
+@[grind .]
+theorem input_convertToLatch
+    (wellFormed : aig.WF)
+    (nextValid : next.validIn aig)
+    (resetAcyclic :
+      match reset with
+      | none => True
+      | some lit => lit.var < idx.getVar aig) :
+    (idx.convertToLatch aig next reset valid varValid).fst.WF := by
+  grind
+
+end input_convertToLatch
+
+/-
+  `InputIdx.convertToAnd`
+-/
+section input_convertToAnd
+variable {idx : InputIdx} {rhs0 rhs1 : Lit}
+variable (valid : idx.validIn aig) (varValid : (idx.getVar aig valid).validIn aig)
+
+@[simp, grind .]
+theorem InputsValid_input_convertToAnd
+    (inputsValid : aig.InputsValid)
+    (h0 : rhs0.var ≠ idx.getVar aig)
+    (h0 : rhs1.var ≠ idx.getVar aig) :
+    (idx.convertToAnd aig rhs0 rhs1 valid varValid).InputsValid := by
+  grind
+
+@[simp, grind .]
+theorem InputIdxsValid_input_convertToAnd
+    (inputIdxsValid : aig.InputIdxsValid)
+    (h0 : rhs0.var ≠ idx.getVar aig)
+    (h0 : rhs1.var ≠ idx.getVar aig) :
+    (idx.convertToAnd aig rhs0 rhs1 valid varValid).InputIdxsValid := by
+  grind
+
+@[simp, grind .]
+theorem LatchesValid_input_convertToAnd
+    (latchesValid : aig.LatchesValid)
+    (inputsValid  : aig.InputsValid)
+    (h0 : rhs0.var ≠ idx.getVar aig)
+    (h0 : rhs1.var ≠ idx.getVar aig) :
+    (idx.convertToAnd aig rhs0 rhs1 valid varValid).LatchesValid := by
+  grind
+
+@[simp, grind .]
+theorem LatchIdxsValid_input_convertToAnd
+    (latchIdxsValid : aig.LatchIdxsValid)
+    (h0 : rhs0.var ≠ idx.getVar aig)
+    (h0 : rhs1.var ≠ idx.getVar aig) :
+    (idx.convertToAnd aig rhs0 rhs1 valid varValid).LatchIdxsValid := by
+  grind
+
+@[simp, grind .]
+theorem ResetsValid_input_convertToAnd
+    (resetsValid : aig.ResetsValid)
+    (h0 : rhs0.var ≠ idx.getVar aig)
+    (h0 : rhs1.var ≠ idx.getVar aig) :
+    (idx.convertToAnd aig rhs0 rhs1 valid varValid).ResetsValid := by
+  grind
+
+@[simp, grind .]
+theorem NextsValid_input_convertToAnd
+    (nextsValid : aig.NextsValid)
+    (h0 : rhs0.var ≠ idx.getVar aig)
+    (h0 : rhs1.var ≠ idx.getVar aig) :
+    (idx.convertToAnd aig rhs0 rhs1 valid varValid).NextsValid := by
+  grind
+
+@[simp, grind .]
+theorem AcyclicGates_input_convertToAnd
+    (acyclicGates : aig.AcyclicGates)
+    (h0 : rhs0.var < idx.getVar aig)
+    (h0 : rhs1.var < idx.getVar aig) :
+    (idx.convertToAnd aig rhs0 rhs1 valid varValid).AcyclicGates := by
+  have : rhs0.var ≠ idx.getVar aig ∧ rhs1.var ≠ idx.getVar aig := by grind
+  grind
+
+@[simp, grind .]
+theorem AcyclicResets_input_convertToAnd
+    (acyclicResets : aig.AcyclicResets) :
+    (idx.convertToAnd aig rhs0 rhs1 valid varValid).AcyclicResets := by
+  grind
+
+@[simp, grind .]
+theorem input_convertToAnd
+    (wellFormed : aig.WF)
+    (h0 : rhs0.var < idx.getVar aig)
+    (h0 : rhs1.var < idx.getVar aig) :
+    (idx.convertToAnd aig rhs0 rhs1 valid varValid).WF := by
+  have : rhs0.var ≠ idx.getVar aig ∧ rhs1.var ≠ idx.getVar aig := by grind
+  grind
+
+end input_convertToAnd
+
+/-
+  `InputIdx.changeIdx`
+-/
+section input_changeIdx
+variable {old new : InputIdx}
+variable (valid : old.validIn aig) (varValid : (old.getVar aig).validIn aig) (unused : ¬new.validIn aig ∨ old = new)
+
+@[simp, grind .]
+theorem InputsValid_input_changeIdx
+    (inputsValid : aig.InputsValid) :
+    (old.changeIdx new aig valid varValid unused).InputsValid := by
+  grind
+
+@[simp, grind .]
+theorem InputIdxsValid_input_changeIdx
+    (inputIdxsValid : aig.InputIdxsValid) :
+    (old.changeIdx new aig valid varValid unused).InputIdxsValid := by
+  grind
+
+@[simp, grind .]
+theorem LatchesValid_input_changeIdx
+    (latchesValid : aig.LatchesValid)
+    (inputsValid : aig.InputsValid) :
+    (old.changeIdx new aig valid varValid unused).LatchesValid := by
+  grind
+
+@[simp, grind .]
+theorem LatchIdxsValid_input_changeIdx
+    (latchIdxsValid : aig.LatchIdxsValid) :
+    (old.changeIdx new aig valid varValid unused).LatchIdxsValid := by
+  grind
+
+@[simp, grind .]
+theorem ResetsValid_input_changeIdx
+    (resetsValid : aig.ResetsValid) :
+    (old.changeIdx new aig valid varValid unused).ResetsValid := by
+  grind
+
+@[simp, grind .]
+theorem NextsValid_input_changeIdx
+    (nextsValid : aig.NextsValid) :
+    (old.changeIdx new aig valid varValid unused).NextsValid := by
+  grind
+
+@[simp, grind .]
+theorem AcyclicGates_input_changeIdx
+    (acyclicGates : aig.AcyclicGates) :
+    (old.changeIdx new aig valid varValid unused).AcyclicGates := by
+  grind
+
+@[simp, grind .]
+theorem AcyclicResets_input_changeIdx
+    (acyclicResets : aig.AcyclicResets) :
+    (old.changeIdx new aig valid varValid unused).AcyclicResets := by
+  grind
+
+@[simp, grind .]
+theorem input_changeIdx
+    (wellFormed : aig.WF) :
+    (old.changeIdx new aig valid varValid unused).WF := by
+  grind
+
+end input_changeIdx
+
+/-
+  `LatchIdx.convertToInput`
+-/
+section latch_convertToInput
+variable {idx : LatchIdx}
+variable (valid : idx.validIn aig) (varValid : (idx.getVar aig valid).validIn aig)
+
+@[simp, grind .]
+theorem InputsValid_latch_convertToInput
+    (inputsValid : aig.InputsValid)
+    (latchesValid : aig.LatchesValid) :
+    (idx.convertToInput aig valid varValid).fst.InputsValid := by
+  grind
+
+@[simp, grind .]
+theorem InputIdxsValid_latch_convertToInput
+    (inputIdxsValid : aig.InputIdxsValid) :
+    (idx.convertToInput aig valid varValid).fst.InputIdxsValid := by
+  grind
+
+@[simp, grind .]
+theorem LatchesValid_latch_convertToInput
+    (latchesValid : aig.LatchesValid) :
+    (idx.convertToInput aig valid varValid).fst.LatchesValid := by
+  grind
+
+@[simp, grind .]
+theorem LatchIdxsValid_latch_convertToInput
+    (latchIdxsValid : aig.LatchIdxsValid) :
+    (idx.convertToInput aig valid varValid).fst.LatchIdxsValid := by
+  grind
+
+@[simp, grind .]
+theorem ResetsValid_latch_convertToInput
+    (resetsValid : aig.ResetsValid) :
+    (idx.convertToInput aig valid varValid).fst.ResetsValid := by
+  grind
+
+@[simp, grind .]
+theorem NextsValid_latch_convertToInput
+    (nextsValid : aig.NextsValid) :
+    (idx.convertToInput aig valid varValid).fst.NextsValid := by
+  grind
+
+@[simp, grind .]
+theorem AcyclicGates_latch_convertToInput
+    (acyclicGates : aig.AcyclicGates) :
+    (idx.convertToInput aig valid varValid).fst.AcyclicGates := by
+  grind
+
+@[simp, grind .]
+theorem AcyclicResets_latch_convertToInput
+    (acyclicResets : aig.AcyclicResets) :
+    (idx.convertToInput aig valid varValid).fst.AcyclicResets := by
+  grind
+
+@[simp, grind .]
+theorem latch_convertToInput
+    (wellFormed : aig.WF) :
+    (idx.convertToInput aig valid varValid).fst.WF := by
+  grind
+
+end latch_convertToInput
+
+/-
+  `LatchIdx.convertToAnd`
+-/
+section latch_convertToAnd
+variable {idx : LatchIdx} {rhs0 rhs1 : Lit}
+variable (valid : idx.validIn aig) (varValid : (idx.getVar aig valid).validIn aig)
+
+@[simp, grind .]
+theorem InputsValid_latch_convertToAnd
+    (inputsValid : aig.InputsValid)
+    (latchesValid : aig.LatchesValid)
+    (h0 : rhs0.var ≠ idx.getVar aig)
+    (h0 : rhs1.var ≠ idx.getVar aig) :
+    (idx.convertToAnd aig rhs0 rhs1 valid varValid).InputsValid := by
+  grind
+
+@[simp, grind .]
+theorem InputIdxsValid_latch_convertToAnd
+    (inputIdxsValid : aig.InputIdxsValid)
+    (h0 : rhs0.var ≠ idx.getVar aig)
+    (h0 : rhs1.var ≠ idx.getVar aig) :
+    (idx.convertToAnd aig rhs0 rhs1 valid varValid).InputIdxsValid := by
+  grind
+
+@[simp, grind .]
+theorem LatchesValid_latch_convertToAnd
+    (latchesValid : aig.LatchesValid)
+    (h0 : rhs0.var ≠ idx.getVar aig)
+    (h0 : rhs1.var ≠ idx.getVar aig) :
+    (idx.convertToAnd aig rhs0 rhs1 valid varValid).LatchesValid := by
+  grind
+
+@[simp, grind .]
+theorem LatchIdxsValid_latch_convertToAnd
+    (latchIdxsValid : aig.LatchIdxsValid)
+    (h0 : rhs0.var ≠ idx.getVar aig)
+    (h0 : rhs1.var ≠ idx.getVar aig) :
+    (idx.convertToAnd aig rhs0 rhs1 valid varValid).LatchIdxsValid := by
+  grind
+
+@[simp, grind .]
+theorem ResetsValid_latch_convertToAnd
+    (resetsValid : aig.ResetsValid)
+    (h0 : rhs0.var ≠ idx.getVar aig)
+    (h0 : rhs1.var ≠ idx.getVar aig) :
+    (idx.convertToAnd aig rhs0 rhs1 valid varValid).ResetsValid := by
+  grind
+
+@[simp, grind .]
+theorem NextsValid_latch_convertToAnd
+    (nextsValid : aig.NextsValid)
+    (h0 : rhs0.var ≠ idx.getVar aig)
+    (h0 : rhs1.var ≠ idx.getVar aig) :
+    (idx.convertToAnd aig rhs0 rhs1 valid varValid).NextsValid := by
+  grind
+
+@[simp, grind .]
+theorem AcyclicGates_latch_convertToAnd
+    (acyclicGates : aig.AcyclicGates)
+    (h0 : rhs0.var < idx.getVar aig)
+    (h0 : rhs1.var < idx.getVar aig) :
+    (idx.convertToAnd aig rhs0 rhs1 valid varValid).AcyclicGates := by
+  have : rhs0.var ≠ idx.getVar aig ∧ rhs1.var ≠ idx.getVar aig := by grind
+  grind
+
+@[simp, grind .]
+theorem AcyclicResets_latch_convertToAnd
+    (acyclicResets : aig.AcyclicResets) :
+    (idx.convertToAnd aig rhs0 rhs1 valid varValid).AcyclicResets := by
+  grind
+
+@[simp, grind .]
+theorem latch_convertToAnd
+    (wellFormed : aig.WF)
+    (h0 : rhs0.var < idx.getVar aig)
+    (h0 : rhs1.var < idx.getVar aig) :
+    (idx.convertToAnd aig rhs0 rhs1 valid varValid).WF := by
+  have : rhs0.var ≠ idx.getVar aig ∧ rhs1.var ≠ idx.getVar aig := by grind
+  grind
+
+end latch_convertToAnd
+
+/-
+  `LatchIdx.changeIdx`
+-/
+section latch_changeIdx
+variable {old new : LatchIdx}
+variable (valid : old.validIn aig) (varValid : (old.getVar aig).validIn aig) (unused : ¬new.validIn aig ∨ old = new)
+
+@[simp, grind .]
+theorem InputsValid_latch_changeIdx
+    (inputsValid : aig.InputsValid)
+    (latchesValid : aig.LatchesValid) :
+    (old.changeIdx new aig valid varValid unused).InputsValid := by
+  grind
+
+@[simp, grind .]
+theorem InputIdxsValid_latch_changeIdx
+    (inputIdxsValid : aig.InputIdxsValid) :
+    (old.changeIdx new aig valid varValid unused).InputIdxsValid := by
+  grind
+
+@[simp, grind .]
+theorem LatchesValid_latch_changeIdx
+    (latchesValid : aig.LatchesValid) :
+    (old.changeIdx new aig valid varValid unused).LatchesValid := by
+  grind
+
+@[simp, grind .]
+theorem LatchIdxsValid_latch_changeIdx
+    (latchIdxsValid : aig.LatchIdxsValid) :
+    (old.changeIdx new aig valid varValid unused).LatchIdxsValid := by
+  grind
+
+@[simp, grind .]
+theorem ResetsValid_latch_changeIdx
+    (resetsValid : aig.ResetsValid) :
+    (old.changeIdx new aig valid varValid unused).ResetsValid := by
+  grind
+
+@[simp, grind .]
+theorem NextsValid_latch_changeIdx
+    (nextsValid : aig.NextsValid) :
+    (old.changeIdx new aig valid varValid unused).NextsValid := by
+  grind
+
+@[simp, grind .]
+theorem AcyclicGates_latch_changeIdx
+    (acyclicGates : aig.AcyclicGates) :
+    (old.changeIdx new aig valid varValid unused).AcyclicGates := by
+  grind
+
+@[simp, grind .]
+theorem AcyclicResets_latch_changeIdx
+    (acyclicResets : aig.AcyclicResets) :
+    (old.changeIdx new aig valid varValid unused).AcyclicResets := by
+  grind
+
+@[simp, grind .]
+theorem latch_changeIdx
+    (wellFormed : aig.WF) :
+    (old.changeIdx new aig valid varValid unused).WF := by
+  grind
+
+end latch_changeIdx
+
+/-
+  `convertAndToInput`
+-/
+section convertAndToInput
+variable {var : Var} (valid : var.validIn aig)
+
+@[simp, grind .]
+theorem InputsValid_convertAndToInput isAnd
+    (inputsValid : aig.InputsValid) :
+    (aig.convertAndToInput var valid isAnd).fst.InputsValid := by
+  grind
+
+@[simp, grind .]
+theorem InputIdxsValid_convertAndToInput isAnd
+    (inputIdxsValid : aig.InputIdxsValid) :
+    (aig.convertAndToInput var valid isAnd).fst.InputIdxsValid := by
+  grind
+
+@[simp, grind .]
+theorem LatchesValid_convertAndToInput isAnd
+    (latchesValid : aig.LatchesValid) :
+    (aig.convertAndToInput var valid isAnd).fst.LatchesValid := by
+  grind
+
+@[simp, grind .]
+theorem LatchIdxsValid_convertAndToInput isAnd
+    (latchIdxsValid : aig.LatchIdxsValid) :
+    (aig.convertAndToInput var valid isAnd).fst.LatchIdxsValid := by
+  grind
+
+@[simp, grind .]
+theorem ResetsValid_convertAndToInput isAnd
+    (resetsValid : aig.ResetsValid) :
+    (aig.convertAndToInput var valid isAnd).fst.ResetsValid := by
+  grind
+
+@[simp, grind .]
+theorem NextsValid_convertAndToInput isAnd
+    (nextsValid : aig.NextsValid) :
+    (aig.convertAndToInput var valid isAnd).fst.NextsValid := by
+  grind
+
+@[simp, grind .]
+theorem AcyclicGates_convertAndToInput isAnd
+    (acyclicGates : aig.AcyclicGates) :
+    (aig.convertAndToInput var valid isAnd).fst.AcyclicGates := by
+  grind
+
+@[simp, grind .]
+theorem AcyclicResets_convertAndToInput isAnd
+    (acyclicResets : aig.AcyclicResets) :
+    (aig.convertAndToInput var valid isAnd).fst.AcyclicResets := by
+  grind
+
+@[simp, grind .]
+theorem convertAndToInput isAnd
+    (wellFormed : aig.WF) :
+    (aig.convertAndToInput var valid isAnd).fst.WF := by
+  grind
+
+end convertAndToInput
+
+/-
+  `convertAndToLatch`
+-/
+section convertAndToLatch
+variable {var : Var} {next : Lit} {reset : Option Lit} (valid : var.validIn aig)
+
+@[simp, grind .]
+theorem InputsValid_convertAndToLatch isAnd
+    (inputsValid : aig.InputsValid) :
+    (aig.convertAndToLatch var next reset valid isAnd).fst.InputsValid := by
+  grind
+
+@[simp, grind .]
+theorem InputIdxsValid_convertAndToLatch isAnd
+    (inputIdxsValid : aig.InputIdxsValid) :
+    (aig.convertAndToLatch var next reset valid isAnd).fst.InputIdxsValid := by
+  grind
+
+@[simp, grind .]
+theorem LatchesValid_convertAndToLatch isAnd
+    (latchesValid : aig.LatchesValid) :
+    (aig.convertAndToLatch var next reset valid isAnd).fst.LatchesValid := by
+  grind
+
+@[simp, grind .]
+theorem LatchIdxsValid_convertAndToLatch isAnd
+    (latchIdxsValid : aig.LatchIdxsValid) :
+    (aig.convertAndToLatch var next reset valid isAnd).fst.LatchIdxsValid := by
+  grind
+
+@[simp]
+theorem ResetsValid_convertAndToLatch_none isAnd
+    (resetsValid : aig.ResetsValid) :
+    (aig.convertAndToLatch var next none valid isAnd).fst.ResetsValid := by
+  grind
+
+@[simp]
+theorem ResetsValid_convertAndToLatch_some isAnd {reset : Lit}
+    (resetsValid : aig.ResetsValid)
+    (resetValid : reset.validIn aig) :
+    (aig.convertAndToLatch var next reset valid isAnd).fst.ResetsValid := by
+  grind
+
+@[grind .]
+theorem ResetsValid_convertAndToLatch isAnd
+    (resetsValid : aig.ResetsValid)
+    (resetValid :
+      match reset with
+      | none => True
+      | some lit => lit.validIn aig) :
+    (aig.convertAndToLatch var next reset valid isAnd).fst.ResetsValid := by
+  grind
+
+@[simp, grind .]
+theorem NextsValid_convertAndToLatch isAnd
+    (nextsValid : aig.NextsValid)
+    (nextValid : next.validIn aig) :
+    (aig.convertAndToLatch var next reset valid isAnd).fst.NextsValid := by
+  grind
+
+@[simp, grind .]
+theorem AcyclicGates_convertAndToLatch isAnd
+    (acyclicGates : aig.AcyclicGates) :
+    (aig.convertAndToLatch var next reset valid isAnd).fst.AcyclicGates := by
+  grind
+
+@[simp]
+theorem AcyclicResets_convertAndToLatch_none isAnd
+    (acyclicResets : aig.AcyclicResets) :
+    (aig.convertAndToLatch var next none valid isAnd).fst.AcyclicResets := by
+  grind
+
+@[simp]
+theorem AcyclicResets_convertAndToLatch_some isAnd {reset : Lit}
+    (acyclicResets : aig.AcyclicResets)
+    (resetAcyclic : reset.var < var) :
+    (aig.convertAndToLatch var next reset valid isAnd).fst.AcyclicResets := by
+  grind
+
+@[grind .]
+theorem AcyclicResets_convertAndToLatch isAnd
+    (acyclicResets : aig.AcyclicResets)
+    (resetAcyclic :
+      match reset with
+      | none => True
+      | some lit => lit.var < var) :
+    (aig.convertAndToLatch var next reset valid isAnd).fst.AcyclicResets := by
+  grind
+
+@[simp]
+theorem convertAndToLatch_none isAnd
+    (wellFormed : aig.WF)
+    (nextValid : next.validIn aig) :
+    (aig.convertAndToLatch var next none valid isAnd).fst.WF := by
+  grind
+
+@[simp]
+theorem convertAndToLatch_some isAnd {reset : Lit}
+    (wellFormed : aig.WF)
+    (nextValid : next.validIn aig)
+    (resetAcyclic : reset.var < var) :
+    (aig.convertAndToLatch var next reset valid isAnd).fst.WF := by
+  grind
+
+@[grind .]
+theorem convertAndToLatch isAnd
+    (wellFormed : aig.WF)
+    (nextValid : next.validIn aig)
+    (resetAcyclic :
+      match reset with
+      | none => True
+      | some lit => lit.var < var) :
+    (aig.convertAndToLatch var next reset valid isAnd).fst.WF := by
+  grind
+
+end convertAndToLatch
+
+/-
+  `rewriteAnd`
+-/
+section rewriteAnd
+variable {var : Var} {rhs0 rhs1 : Lit} (valid : var.validIn aig)
+
+@[simp, grind .]
+theorem InputsValid_rewriteAnd isAnd
+    (inputsValid : aig.InputsValid)
+    (h0 : rhs0.var ≠ var)
+    (h0 : rhs1.var ≠ var) :
+    (aig.rewriteAnd var rhs0 rhs1 valid isAnd).InputsValid := by
+  grind
+
+@[simp, grind .]
+theorem InputIdxsValid_rewriteAnd isAnd
+    (inputIdxsValid : aig.InputIdxsValid)
+    (h0 : rhs0.var ≠ var)
+    (h0 : rhs1.var ≠ var) :
+    (aig.rewriteAnd var rhs0 rhs1 valid isAnd).InputIdxsValid := by
+  grind
+
+@[simp, grind .]
+theorem LatchesValid_rewriteAnd isAnd
+    (latchesValid : aig.LatchesValid)
+    (h0 : rhs0.var ≠ var)
+    (h0 : rhs1.var ≠ var) :
+    (aig.rewriteAnd var rhs0 rhs1 valid isAnd).LatchesValid := by
+  grind
+
+@[simp, grind .]
+theorem LatchIdxsValid_rewriteAnd isAnd
+    (latchIdxsValid : aig.LatchIdxsValid)
+    (h0 : rhs0.var ≠ var)
+    (h0 : rhs1.var ≠ var) :
+    (aig.rewriteAnd var rhs0 rhs1 valid isAnd).LatchIdxsValid := by
+  grind
+
+@[simp, grind .]
+theorem ResetsValid_rewriteAnd isAnd
+    (resetsValid : aig.ResetsValid)
+    (h0 : rhs0.var ≠ var)
+    (h0 : rhs1.var ≠ var) :
+    (aig.rewriteAnd var rhs0 rhs1 valid isAnd).ResetsValid := by
+  grind
+
+@[simp, grind .]
+theorem NextsValid_rewriteAnd isAnd
+    (nextsValid : aig.NextsValid)
+    (h0 : rhs0.var ≠ var)
+    (h0 : rhs1.var ≠ var) :
+    (aig.rewriteAnd var rhs0 rhs1 valid isAnd).NextsValid := by
+  grind
+
+@[simp, grind .]
+theorem AcyclicGates_rewriteAnd isAnd
+    (acyclicGates : aig.AcyclicGates)
+    (h0 : rhs0.var < var)
+    (h0 : rhs1.var < var) :
+    (aig.rewriteAnd var rhs0 rhs1 valid isAnd).AcyclicGates := by
+  have : rhs0.var ≠ var ∧ rhs1.var ≠ var := by grind
+  grind
+
+@[simp, grind .]
+theorem AcyclicResets_rewriteAnd isAnd
+    (acyclicResets : aig.AcyclicResets) :
+    (aig.rewriteAnd var rhs0 rhs1 valid isAnd).AcyclicResets := by
+  grind
+
+@[simp, grind .]
+theorem rewriteAnd isAnd
+    (wellFormed : aig.WF)
+    (h0 : rhs0.var < var)
+    (h0 : rhs1.var < var) :
+    (aig.rewriteAnd var rhs0 rhs1 valid isAnd).WF := by
+  have : rhs0.var ≠ var ∧ rhs1.var ≠ var := by grind
+  grind
+
+end rewriteAnd
+
+end WF
+
+end Valaig.Aig
