Valaig/Prelude.lean
@@ -1,8 +1,5 @@
 module
 
-public import Lean.Meta.Tactic.Grind.RegisterCommand
-public import Lean.Meta.Tactic.Simp.RegisterCommand
-
 namespace Valaig
 
 scoped macro:50 "rlet" pat:term ":=" expr:term rest:term : term =>
@@ -24,15 +21,6 @@ scoped macro:50 "rlet" h:ident ":" pat:term "←" expr:term  rest:term : term =>
       | some $pat => $rest)
 
 namespace Aig
-
-register_grind_attr grind_valaig_defs
-register_simp_attr simp_valaig_defs
-
-scoped macro "simp_defs" : tactic => `(tactic| (simp [simp_valaig_defs]))
-scoped macro "simp_all_defs" : tactic => `(tactic| (simp_all [simp_valaig_defs]))
-
-set_option hygiene false in
-scoped macro "grind_defs" : tactic => `(tactic| (grind [grind_valaig_defs]))
 
 scoped macro_rules
 | `(tactic| get_elem_tactic_extensible) => `(tactic| grind)
