Valaig/Utils/Map.lean
@@ -1,0 +1,522 @@
+module
+
+public import Valaig.Utils.Pool
+
+public section
+namespace Valaig.Utils
+
+@[ext]
+structure Map (α : Type) (β : Type) [DecidableEq α] where
+  raw ::
+    valid : α -> Prop
+    _decide : α -> Bool
+    _decideLegal (key : α) : valid key ↔ _decide key = true
+    map (key : α) (h : valid key) : β
+    size : Nat
+
+namespace Map
+variable {α : Type}
+
+class AsNat (α : Type) where
+  toNat : α -> Nat
+  ofNat : Nat -> α
+  ofNat_toNat : ∀ key, ofNat (toNat key) = key := by grind
+  toNat_ofNat : ∀ n, toNat (ofNat n) = n := by grind
+
+attribute [simp, grind =] AsNat.ofNat_toNat AsNat.toNat_ofNat
+attribute [simp] AsNat.toNat AsNat.ofNat
+
+variable [DecidableEq α] {β : Type} {map : Map α β} {key : α} {value : β}
+
+private theorem hfunext {α α' : Sort u} {β : α → Sort v} {β' : α' → Sort v} {f : ∀ a, β a} {f' : ∀ a, β' a}
+    (hα : α = α') (h : ∀ a a', a ≍ a' → f a ≍ f' a') : f ≍ f' := by
+  subst hα
+  have : ∀ a, f a ≍ f' a := fun a ↦ h a a (HEq.refl a)
+  have : β = β' := by funext a; exact type_eq_of_heq (this a)
+  subst this
+  grind
+
+theorem ext' (a b : Map α β)
+    (valid : ∀ key, a.valid key = b.valid key)
+    (map : ∀ key h, a.map key h = b.map key (by grind))
+    (size : a.size = b.size) :
+    a = b := by
+  apply Map.ext
+  · grind
+  · have := a._decideLegal
+    have := b._decideLegal
+    grind
+  · apply hfunext
+    · grind
+    · intros
+      apply hfunext
+      · grind
+      · grind
+  · grind
+
+@[always_inline]
+instance : Membership α (Map α β) where
+  mem map key := map.valid key
+
+@[always_inline]
+instance : Decidable (map.valid key) :=
+  have : map.valid key ↔ map._decide key := by simp [map._decideLegal]
+  decidable_of_iff' _ this
+
+@[always_inline]
+instance : Decidable (key ∈ map) := by
+  simp +instances only [instMembership]
+  infer_instance
+
+@[local grind =_]
+theorem valid_iff :
+    map.valid key ↔ key ∈ map := by
+  rfl
+
+@[always_inline]
+instance : GetElem (Map α β) α β (fun map key => key ∈ map) where
+  getElem := Map.map
+
+@[local grind =_]
+theorem map_eq (h : key ∈ map) :
+    map.map key h = map[key]:= by
+  rfl
+
+structure Monotone (old new : Map α β) : Prop where
+  valid (key : α) : old.valid key → new.valid key
+  map (key : α) (h : old.valid key) : old.map key h = new.map key (valid key h)
+  sized : old.size ≤ new.size
+
+@[always_inline]
+instance : LE (Map α β) where
+  le := Monotone
+
+@[simp, grind =]
+theorem mono_iff {old new : Map α β} :
+    old.Monotone new ↔ old ≤ new := by
+  rfl
+
+instance : Std.IsPreorder (Map α β) := by
+  apply Std.IsPreorder.of_le
+  <;> constructor
+  · intros; constructor <;> simp
+  · simp only [←mono_iff]; intros; constructor <;> grind only [Monotone]
+
+section Monotone
+variable {old new : Map α β}
+
+@[simp, grind .]
+theorem mem_mono (mono : old ≤ new) (h : key ∈ old) :
+    key ∈ new := by
+  grind [mono.valid]
+
+@[simp]
+theorem getElem_mono (mono : old ≤ new) (h : key ∈ old) {h' : key ∈ new} :
+    new[key]'h' = old[key] := by
+  grind [mono.map]
+
+grind_pattern getElem_mono => new[key], old ≤ new
+
+@[simp, grind .]
+theorem size_mono (mono : old ≤ new) :
+    old.size ≤ new.size :=
+  mono.sized
+
+end Monotone
+
+@[expose]
+def mk (valid : α -> Prop) (map : (key : α) -> valid key -> β) (size : Nat) [DecidablePred valid] : Map α β where
+  valid := valid
+  _decide key := Decidable.decide (valid key)
+  _decideLegal := by grind
+  map := map
+  size := size
+
+section mk
+variable {valid : α -> Prop} {map : (key : α) -> valid key -> β} {size : Nat} [DecidablePred valid]
+
+@[simp, grind =]
+theorem valid_mk :
+    (mk valid map size).valid = valid := by
+  rfl
+
+@[simp, grind =]
+theorem map_mk :
+    (mk valid map size).map = map := by
+  rfl
+
+@[simp, grind =]
+theorem size_mk :
+    (mk valid map size).size = size := by
+  rfl
+
+@[simp, grind =]
+theorem mem_mk :
+    key ∈ (mk valid map size) ↔ valid key := by
+  rfl
+
+@[simp, grind =]
+theorem getElem_mk (mem : key ∈ mk valid map size) :
+    (mk valid map size)[key]'mem = map key mem := by
+  rfl
+
+end mk
+
+def empty : Map α β :=
+  .mk
+    (valid := fun _ => False)
+    (map := by grind)
+    (size := 0)
+
+section empty
+attribute [local simp, local grind] empty
+
+@[simp, grind =]
+theorem size_empty :
+    (empty : Map α β).size = 0 := by
+  grind
+
+@[simp, grind .]
+theorem mem_empty :
+    key ∉ (empty : Map α β) := by
+  grind
+
+@[simp, grind .]
+theorem mono_empty (new : Map α β) :
+    empty ≤ new := by
+  constructor <;> grind
+
+end empty
+
+set_option linter.unusedVariables false in
+def push (map : Map α β) (key : α) (value : β) (new : key ∉ map := by grind) : Map α β :=
+  .mk
+    (valid := fun key' => key' ∈ map ∨ key = key')
+    (map := fun key _ => if h : key ∈ map then map[key] else value)
+    (size := map.size + 1)
+
+section push
+variable {key : α} {value : β} (new : key ∉ map)
+attribute [local simp, local grind] push
+
+@[simp, grind =]
+theorem size_push :
+    (map.push key value new).size = map.size + 1 := by
+  grind
+
+@[simp]
+theorem mem_push_old {old : α} (h : old ∈ map) :
+    old ∈ (map.push key value new) := by
+  grind
+
+@[simp]
+theorem mem_push_self :
+    key ∈ (map.push key value new) := by
+  grind
+
+@[simp, grind =]
+theorem mem_push {key' : α} :
+    key' ∈ (map.push key value new) ↔
+    key' ∈ map ∨ key' = key := by
+  grind
+
+@[simp]
+theorem getElem_push_old {old : α} (mem : old ∈ map) :
+    (map.push key value new)[old]'(by grind) = map[old] := by
+  grind
+
+@[simp]
+theorem getElem_push_self :
+    (map.push key value new)[key] = value := by
+  grind
+
+@[simp, grind =]
+theorem getElem_push {key' : α} (mem : key' ∈ map.push key value new) :
+    (map.push key value new)[key'] =
+    if _ : key' = key then value else map[key']'(by grind) := by
+  grind
+
+@[simp, grind! .]
+theorem mono_push :
+    map ≤ map.push key value new := by
+  constructor <;> grind [push]
+
+end push
+
+def insert (map : Map α β) (key : α) (value : β) : Map α β :=
+  .mk
+    (valid := fun key' => key' ∈ map ∨ key' = key)
+    (map := fun key' _ => if _ : key' = key then value else map[key']'(by grind))
+    (size := if key ∈ map then map.size else map.size + 1)
+
+section insert
+variable {key : α} {value : β}
+attribute [local simp, local grind] insert
+
+@[simp]
+theorem size_insert_mem (mem : key ∈ map) :
+    (map.insert key value).size = map.size := by
+  grind
+
+@[simp]
+theorem size_insert_not_mem (notmem : key ∉ map) :
+    (map.insert key value).size = map.size + 1 := by
+  grind
+
+@[simp, grind =]
+theorem size_insert :
+    (map.insert key value).size = if key ∈ map then map.size else map.size + 1 := by
+  grind
+
+@[simp]
+theorem mem_insert_old {old : α} (h : old ∈ map) :
+    old ∈ (map.insert key value) := by
+  grind
+
+@[simp]
+theorem mem_insert_self :
+    key ∈ (map.insert key value) := by
+  grind
+
+@[simp, grind =]
+theorem mem_insert {key' : α} :
+    key' ∈ (map.insert key value) ↔
+    key' ∈ map ∨ key' = key := by
+  grind
+
+@[simp]
+theorem getElem_insert_old_not_mem {old : α} (mem : old ∈ map) (notmem : key ∉ map) :
+    (map.insert key value)[old]'(by grind) = map[old] := by
+  grind
+
+@[simp]
+theorem getElem_insert_self :
+    (map.insert key value)[key] = value := by
+  grind
+
+@[simp, grind =]
+theorem getElem_insert {key' : α} (mem : key' ∈ map.insert key value) :
+    (map.insert key value)[key'] =
+    if _ : key' = key then value else map[key']'(by grind) := by
+  grind
+
+@[simp, grind! .]
+theorem mono_insert (unused : key ∉ map) :
+    map ≤ map.insert key value := by
+  constructor <;> grind
+
+@[simp, grind =]
+theorem insert_eq_push  (new : key ∉ map) :
+    map.insert key value = map.push key value := by
+  unfold insert push
+  apply ext' <;> grind
+
+end insert
+
+set_option linter.unusedVariables false in
+def set (map : Map α β) (key : α) (value : β) (mem : key ∈ map := by grind) : Map α β :=
+  { map with map key' _ := if key' = key then value else map[key'] }
+
+section set
+variable {key : α} {value : β} (mem : key ∈ map)
+attribute [local simp, local grind] set
+
+@[simp, grind =]
+theorem size_set :
+    (map.set key value mem).size = map.size := by
+  grind
+
+@[simp, grind =]
+theorem mem_set {key' : α} :
+    key' ∈ (map.set key value mem) ↔ key' ∈ map := by
+  grind
+
+@[simp]
+theorem getElem_set_self :
+    (map.set key value mem)[key] = value := by
+  grind
+
+@[simp, grind =]
+theorem getElem_set {key' : α} (mem' : key' ∈ map.set key value mem) :
+    (map.set key value mem)[key'] =
+    have h : key' ∈ map := by grind
+    if _ : key' = key then value else map[key']'h := by
+  unfold set
+  grind
+
+end set
+
+def modify (map : Map α β) (key : α) (f : β -> β) : Map α β :=
+  { map with map key' _ := if key' = key then f map[key'] else map[key'] }
+
+section modify
+variable {key : α} (f : β -> β)
+attribute [local simp, local grind] modify
+
+@[simp, grind =]
+theorem size_modify :
+    (map.modify key f).size = map.size := by
+  grind
+
+@[simp, grind =]
+theorem mem_modify {key' : α} :
+    key' ∈ (map.modify key f) ↔ key' ∈ map := by
+  grind
+
+@[simp]
+theorem getElem_modify_self (mem : key ∈ map) :
+    (map.modify key f)[key] = f map[key] := by
+  grind
+
+@[simp, grind =]
+theorem getElem_modify {key' : α} (mem' : key' ∈ map.modify key f) :
+    (map.modify key f)[key'] =
+    have h : key' ∈ map := by grind
+    if _ : key' = key then f (map[key']'h) else (map[key']'h) := by
+  unfold modify
+  grind
+
+end modify
+
+def erase (map : Map α β) (key : α) : Map α β :=
+  .mk
+    (valid := fun key' => key ≠ key' ∧ map.valid key')
+    (map := fun key' _ => map[key']'(by grind))
+    (size := if key ∈ map then map.size - 1 else map.size)
+
+section erase
+variable {key : α}
+attribute [local simp, local grind] erase
+
+@[simp, grind =]
+theorem size_erase :
+    (map.erase key).size = if key ∈ map then map.size - 1 else map.size := by
+  grind
+
+@[simp, grind =]
+theorem mem_erase {key' : α} :
+    key' ∈ map.erase key ↔ key' ≠ key ∧ key' ∈ map := by
+  grind
+
+@[simp, grind =]
+theorem getElem_erase {key' : α} (mem' : key' ∈ map.erase key) :
+    (map.erase key)[key'] =
+    have h : key' ∈ map := by grind
+    map[key']'h := by
+  grind
+
+end erase
+
+def mapVal {γ : Type} (map : Map α β) (f : β -> γ) : Map α γ :=
+  .mk
+    (valid := map.valid)
+    (map := fun key valid => f map[key])
+    (size := map.size)
+
+section mapVal
+variable {γ : Type} {f : β -> γ} {key : α} {value : β}
+attribute [local simp, local grind] mapVal
+
+@[simp, grind =]
+theorem size_mapVal :
+    (map.mapVal f).size = map.size := by
+  grind 
+
+@[simp, grind =]
+theorem mem_mapVal :
+    key ∈ (map.mapVal f) ↔ key ∈ map := by
+  grind 
+
+@[simp, grind =]
+theorem getElem_mapVal (mem : key ∈ map.mapVal f) :
+    (map.mapVal f)[key] =
+    have h : key ∈ map := by grind
+    f map[key] := by
+  grind
+
+@[simp, grind =]
+theorem mapVal_empty :
+    (empty : Map α β).mapVal f = (empty : Map α γ) := by
+  unfold mapVal empty
+  apply ext' <;> grind
+
+@[simp, grind =]
+theorem mapVal_push (new : key ∉ map) :
+    (map.push key value).mapVal f = (map.mapVal f).push key (f value) := by
+  unfold mapVal push
+  apply ext' <;> grind
+
+@[simp, grind =]
+theorem mapVal_insert :
+    (map.insert key value).mapVal f = (map.mapVal f).insert key (f value) := by
+  unfold mapVal insert
+  apply ext' <;> grind
+
+@[simp, grind =]
+theorem mapVal_set (mem : key ∈ map) :
+    (map.set key value).mapVal f = (map.mapVal f).set key (f value) := by
+  unfold mapVal set
+  apply ext' <;> grind
+
+@[simp, grind =]
+theorem mapVal_erase :
+    (map.erase key).mapVal f = (map.mapVal f).erase key := by
+  unfold mapVal erase
+  apply ext' <;> grind
+
+end mapVal
+
+@[always_inline, expose]
+def ofPool (pool : Pool β) (α : Type) [AsNat α] [DecidableEq α] : Map α β :=
+  .mk
+    (valid := (AsNat.toNat · ∈ pool))
+    (map := fun key valid => pool[AsNat.toNat key]'(by grind))
+    (size := pool.size)
+
+section ofPool
+variable {pool : Pool β} [AsNat α]
+
+@[simp, grind =]
+theorem mem_ofPool :
+    key ∈ ofPool pool α ↔ AsNat.toNat key ∈ pool := by
+  rfl
+
+@[simp, grind =]
+theorem getElem_ofPool (mem : key ∈ ofPool pool α) :
+    (ofPool pool α)[key]'mem = pool[AsNat.toNat key] := by
+  rfl
+
+@[simp, grind =]
+theorem size_ofPool :
+    (ofPool pool α).size = pool.size := by
+  rfl
+
+@[simp, grind =]
+theorem ofPool_empty :
+    ofPool (@Pool.empty β) α = .empty := by
+  unfold ofPool empty
+  apply ext' <;> grind
+
+@[simp, grind =]
+theorem ofPool_modify {idx : Nat} (f : β -> β) :
+    ofPool (pool.modify idx f) α = (ofPool pool α).modify (AsNat.ofNat idx) f := by
+  unfold ofPool modify
+  apply ext' <;> grind
+
+@[simp, grind =]
+theorem ofPool_insert {idx : Nat} {val : β} :
+    ofPool (pool.insert idx val) α = (ofPool pool α).insert (AsNat.ofNat idx) val := by
+  unfold ofPool insert
+  apply ext' <;> grind
+
+@[simp, grind =]
+theorem ofPool_erase {idx : Nat} :
+    ofPool (pool.erase idx) α = (ofPool pool α).erase (AsNat.ofNat idx) := by
+  unfold ofPool erase
+  apply ext' <;> grind
+
+end ofPool
+
+attribute [simp, grind =] valid_iff map_eq
+
+end Map
